add: mul demo

theory/JITPer.thy
@@ -14,8 +14,8 @@ theory JITPer
 imports
   Main
   rBPFCommType rBPFSyntax rBPFSem
-  x64Syntax x64Semantics x64Assembler Proof1 Proof2
-  JITState
+  x64Syntax x64Semantics x64Assembler
+  JITState JITPer2Aux
 
 begin
 
@@ -29,13 +29,13 @@ text \<open> return
 definition per_jit_add_reg64_1 :: "bpf_ireg \<Rightarrow> bpf_ireg \<Rightarrow> (nat \<times> u64 \<times> x64_bin) option" where
 "per_jit_add_reg64_1 dst src = (
   let ins = Paddq_rr (bpf_to_x64_reg dst) (bpf_to_x64_reg src) in
-    map_option (\<lambda> l. (1, 1, l)) (x64_encode ins)
+    Some (1, 1, x64_encode ins) 
 )"
 
 definition per_jit_exit :: "(nat \<times> u64 \<times> x64_bin) option" where
 "per_jit_exit = (
   let ins = Pret in
-    map_option (\<lambda> l. (1, 1, l)) (x64_encode ins)
+    Some (1, 1, x64_encode ins) 
 )"
 
 
@@ -44,14 +44,23 @@ definition per_jit_exit :: "(nat \<times> u64 \<times> x64_bin) option" where
    map_option (\<lambda> l. (5, 1, l)) (x64_encodes_func_suffix ins_list)"*)
 
 definition per_jit_mul_reg64::"bpf_ireg \<Rightarrow> bpf_ireg \<Rightarrow> (nat \<times> u64 \<times> x64_bin) option" where
-"per_jit_mul_reg64 dst src \<equiv> let ins_list = case (bpf_to_x64_reg dst) of
-    RAX \<Rightarrow> [Pmovq_rr (bpf_to_x64_reg src) R11, Ppushl_r RDX, Pmulq_r R11, Ppopl RDX]|
-    RDX \<Rightarrow> [Pmovq_rr (bpf_to_x64_reg src) R11, Ppushl_r RAX, Pmovq_rr RAX RDX, Pmulq_r R11, Pmovq_rr RDX RAX, Ppopl RAX]|
-    _   \<Rightarrow> [Pmovq_rr (bpf_to_x64_reg src) R11, Ppushl_r RAX, Pmovq_rr RAX (bpf_to_x64_reg dst), Ppushl_r RDX, Pmulq_r R11, 
-            Ppopl RDX, Pmovq_rr (bpf_to_x64_reg dst) RAX, Ppopl RAX]
-  in map_option (\<lambda> l. (length ins_list, 1, l)) (x64_encodes2 ins_list)"
+"per_jit_mul_reg64 dst src \<equiv> 
+  let ins_list = case (bpf_to_x64_reg dst) of 
+      RAX \<Rightarrow> (x64_encode (Pmovq_rr R11 (bpf_to_x64_reg src))@(x64_encode (Ppushl_r RDX)) @ (x64_encode (Pmulq_r R11)) @ (x64_encode (Ppopl RDX))) |
+      
+      RDX \<Rightarrow> (x64_encode (Pmovq_rr R11 (bpf_to_x64_reg src))@(x64_encode (Ppushl_r RAX)) @ (x64_encode (Pmovq_rr RAX RDX)) 
+                  @ (x64_encode (Pmulq_r R11))@ (x64_encode (Pmovq_rr RDX RAX))@ (x64_encode (Ppopl RAX)))|
+      
+      _   \<Rightarrow> (x64_encode(Pmovq_rr R11 (bpf_to_x64_reg src)))@(x64_encode (Ppushl_r RAX)) @ (x64_encode (Pmovq_rr RAX (bpf_to_x64_reg dst)))
+                  @ (x64_encode (Ppushl_r RDX)) @ (x64_encode (Pmulq_r R11)) @ (x64_encode (Ppopl RDX))
+                  @ (x64_encode (Pmovq_rr (bpf_to_x64_reg dst) RAX)) @ (x64_encode (Ppopl RAX))
+  in let len = case (bpf_to_x64_reg dst) of 
+    RAX \<Rightarrow> 4 |
+    RDX \<Rightarrow> 6 |
+    _ \<Rightarrow> 8
+    in Some (len, 1, ins_list)"
 
-
+                                               
 fun per_jit_ins ::" bpf_instruction \<Rightarrow> (nat \<times> u64 \<times> x64_bin) option" where
 "per_jit_ins bins = (
   case bins of
@@ -98,9 +107,13 @@ definition match_stack :: "regset \<Rightarrow> mem \<Rightarrow> bool" where
 
 text \<open> because jited x64 code may use pop and push to save registers,
 then x64 memory has more info than sbpf memory \<close>
+(*(Mem.loadv mc bm (Vlong addr) = Some v) \<longrightarrow> (Mem.loadv mc xm (Vlong addr) = Some v))*)
 definition match_mem :: "mem \<Rightarrow> mem \<Rightarrow> bool" where
 "match_mem bm xm = (
   \<forall> mc addr v. (Mem.loadv mc bm addr = Some v) \<longrightarrow> (Mem.loadv mc xm addr = Some v))"
+
+definition match_reg :: "reg_map \<Rightarrow> regset \<Rightarrow> bool" where
+  "match_reg rm rs = (\<forall> r. (rm r) = rs (bpf_to_x64_reg r))"
 
 definition match_state :: "sbpf_state \<Rightarrow> x64_state \<Rightarrow> bool" where
 "match_state bst xst = (
@@ -108,7 +121,7 @@ definition match_state :: "sbpf_state \<Rightarrow> x64_state \<Rightarrow> bool
   SBPF_OK pc rs m \<Rightarrow> (
     case xst of
       Next xpc xrs xm \<Rightarrow>
-        (\<forall> r. (rs r) = xrs (bpf_to_x64_reg r)) \<and> \<comment>\<open> for ALU + MEM + Call \<close>
+        match_reg rs xrs \<and> \<comment>\<open> for ALU + MEM + Call \<close>
         match_mem m xm  \<comment>\<open> for MEM + Call \<close> \<and> 
         match_stack xrs xm |
       _ \<Rightarrow> False
@@ -120,37 +133,6 @@ definition match_state :: "sbpf_state \<Rightarrow> x64_state \<Rightarrow> bool
   ) |
   _ \<Rightarrow> False
 )"
-
-lemma x64_sem_add_stuck : 
-" x64_sem (m + n) x64_prog Stuck = xst' \<Longrightarrow>
-  x64_sem n x64_prog (x64_sem m x64_prog Stuck) = xst'"
-  apply (cases m,simp)
-  subgoal for m
-    apply(cases n,simp)
-    by auto
-  done
-
-lemma x64_sem_add: 
-  "x64_sem (m+n) x64_prog xst = xst' \<Longrightarrow>
-    xst = (Next pc rs ms) \<Longrightarrow>
-    \<exists> xst1.
-    x64_sem m x64_prog xst = xst1 \<and> 
-    x64_sem n x64_prog xst1 = xst'"
-  apply (induction m arbitrary: n x64_prog xst xst' pc rs ms)
-  subgoal by simp
-  subgoal for m n x64_prog xst xst' pc rs ms
-    apply simp
-    apply (cases "x64_decode (unat pc) x64_prog"; simp)
-    subgoal by (cases n; simp)
-    subgoal for ins1
-      apply (cases ins1; simp)
-      subgoal for sz ins
-        apply (cases "(exec_instr ins (word_of_nat sz) pc rs ms)"; simp)
-        apply (erule x64_sem_add_stuck)
-        done
-      done
-    done
-  done
 
 lemma sbpf_sem_induct: 
   "sbpf_sem (m+n) prog s = s' \<Longrightarrow>
@@ -222,6 +204,7 @@ lemma aluq_subgoal_rr_aux2:"xins = Paddq_rr (bpf_to_x64_reg dst) (bpf_to_x64_reg
   using aluq_subgoal_rr_aux2_1 by simp
 
 
+
 lemma aluq_subgoal_rr_aux3:"bins = BPF_ALU64 BPF_ADD dst (SOReg src) \<Longrightarrow> 
   sbpf_step prog (SBPF_OK pc rs m) = (SBPF_OK pc' rs' m') \<Longrightarrow> 
   prog!(unat pc) = bins \<Longrightarrow>
@@ -234,73 +217,139 @@ lemma aluq_subgoal_rr_aux3:"bins = BPF_ALU64 BPF_ADD dst (SOReg src) \<Longright
   done
 
 
+lemma reg_r11_consist:"r = (bpf_to_x64_reg dst) \<Longrightarrow> r \<noteq> x64Syntax.R11"
+  apply(cases dst) 
+  by (unfold bpf_to_x64_reg_corr bpf_to_x64_reg_def, simp_all)
+
+lemma reg_rsp_consist:"r = (bpf_to_x64_reg dst) \<Longrightarrow> r \<noteq> x64Syntax.RSP"
+  apply(cases dst) 
+  by (unfold bpf_to_x64_reg_corr bpf_to_x64_reg_def, simp_all)
+
 lemma mulq_subgoal_rr_aux1_1:
-  "xins = [Pmovq_rr (bpf_to_x64_reg src) R11, Ppushl_r RDX, Pmulq_r R11, Ppopl RDX] \<Longrightarrow>
-  Next pc1 reg1 m1 = exec_instr (Pmulq_r (bpf_to_x64_reg src)) sz pc reg m \<Longrightarrow>
-  Next pc2 reg2 m2 = interp3 xins (Next pc reg m) \<Longrightarrow>
-  (bpf_to_x64_reg dst) = RAX \<Longrightarrow>
-  reg1 (bpf_to_x64_reg dst) =  reg2 (bpf_to_x64_reg dst) "
+  "xins = [(3,Pmovq_rr R11 (bpf_to_x64_reg src)), (1,Ppushl_r RAX), (3,Pmovq_rr RAX RDX), (3,Pmulq_r R11), (3,Pmovq_rr RDX RAX), (1,Ppopl RAX)] \<Longrightarrow>
+    exec_instr (snd(xins!0)) (of_nat(fst(xins!0))) pc rs xm = Next pc1 rs1 m1\<and>
+    exec_instr (snd(xins!1)) (of_nat(fst(xins!1))) pc1 rs1 m1 = Next pc2 rs2 m2 \<and>
+    exec_instr (snd(xins!2)) (of_nat(fst(xins!2))) pc2 rs2 m2 = Next pc3 rs3 m3 \<and>
+    exec_instr (snd(xins!3)) (of_nat(fst(xins!3))) pc3 rs3 m3 = Next pc4 rs4 m4 \<and>
+    exec_instr (snd(xins!4)) (of_nat(fst(xins!4))) pc4 rs4 m4 = Next pc5 rs5 m5 \<and> 
+    exec_instr (snd(xins!5)) (of_nat(fst(xins!5))) pc5 rs5 m5 = Next pc6 rs6 m6  \<Longrightarrow>
+   \<forall> r. bpf_to_x64_reg r \<notin> {RDX, RAX} \<longrightarrow> rs (bpf_to_x64_reg r) = rs6 (bpf_to_x64_reg r) "
   apply(unfold exec_instr_def)
-  apply(cases "xins ! 2",simp_all)
+  apply(cases "Pmulq_r (bpf_to_x64_reg src)",simp_all)
   subgoal for x6
-    apply(cases "exec_instr (Pmovq_rr (bpf_to_x64_reg src) REG_SCRATCH) 1 pc reg m",simp_all)
-    subgoal for x11 x12 x13
-      apply(cases "exec_instr (Ppushl_r RDX) 1 x11 x12 x13",simp_all)
-      subgoal for x11a x12a x13a
-        apply(cases "exec_instr (Pmulq_r REG_SCRATCH) 1 x11a x12a x13a",simp_all)
-        subgoal for x11b x12b x13b
-          apply(unfold exec_instr_def)
-          apply(cases "Ppopl RDX",simp_all)
-          subgoal for x4 apply(unfold exec_push_def Let_def)
-            apply(cases "storev M32 x13 (x12 SP - u64_of_memory_chunk M32) (Vlong (x12 RDX))",simp_all)
-            by (simp add: storev_def)
-          done
-        done
+    apply(unfold exec_push_def exec_pop_def exec_ret_def  Let_def) 
+    using store_load_consistency
+    apply(cases "storev M64 m1 (rs1 SP - u64_of_memory_chunk M64) (Vlong (rs1 RAX))",simp_all)
+    apply(cases "loadv M64 m5 (rs5 SP)", simp_all)
+    subgoal for a apply(cases a,simp_all)
+      subgoal for x5 
+        apply(cases M64,simp_all)
+        using store_load_consistency reg_r11_consist reg_rsp_consist by auto
       done
     done
   done
 
 lemma mulq_subgoal_rr_aux1_2:
-     "(bpf_to_x64_reg dst) = RAX \<Longrightarrow>
+     "(bpf_to_x64_reg dst) = RDX \<Longrightarrow>
      bins = BPF_ALU64 BPF_MUL dst (SOReg src) \<Longrightarrow>
-     xins = Pmulq_r (bpf_to_x64_reg src) \<Longrightarrow>
      prog!(unat pc) = bins \<Longrightarrow>
-     sbpf_step prog (SBPF_OK pc rs m) = (SBPF_OK pc' rs' m')  \<Longrightarrow>
-     Next spc' reg' xm' = exec_instr xins sz spc reg xm \<Longrightarrow>
-     reg (bpf_to_x64_reg dst) = rs dst \<Longrightarrow>
-     reg (bpf_to_x64_reg src) = rs src \<Longrightarrow>
-     reg' (bpf_to_x64_reg dst) = (rs' dst)"
-  apply (unfold exec_instr_def step)
-  apply simp
-  apply(cases "prog ! unat pc",simp_all)
-  subgoal for x91 apply(simp split:if_split_asm) 
-    apply(unfold eval_alu_def eval_reg_def,simp_all)
-    by auto
+     sbpf_step prog (SBPF_OK pc reg m) = (SBPF_OK pc' reg' m')  \<Longrightarrow>
+     xins = [(3,Pmovq_rr R11 (bpf_to_x64_reg src)), (1,Ppushl_r RAX), (3,Pmovq_rr RAX RDX), (3,Pmulq_r R11), (3,Pmovq_rr RDX RAX), (1,Ppopl RAX)] \<Longrightarrow>
+    exec_instr (snd(xins!0)) (of_nat(fst(xins!0))) xpc rs xm = Next pc1 rs1 m1\<and>
+    exec_instr (snd(xins!1)) (of_nat(fst(xins!1))) pc1 rs1 m1 = Next pc2 rs2 m2 \<and>
+    exec_instr (snd(xins!2)) (of_nat(fst(xins!2))) pc2 rs2 m2 = Next pc3 rs3 m3 \<and>
+    exec_instr (snd(xins!3)) (of_nat(fst(xins!3))) pc3 rs3 m3 = Next pc4 rs4 m4 \<and>
+    exec_instr (snd(xins!4)) (of_nat(fst(xins!4))) pc4 rs4 m4 = Next pc5 rs5 m5 \<and> 
+    exec_instr (snd(xins!5)) (of_nat(fst(xins!5))) pc5 rs5 m5 = Next pc6 rs6 m6 \<Longrightarrow>
+     rs (bpf_to_x64_reg dst) = reg dst \<Longrightarrow>
+     rs (bpf_to_x64_reg src) = reg src \<Longrightarrow>
+     rs6 (bpf_to_x64_reg dst) = (reg' dst)"
+    apply (unfold exec_instr_def step) 
+    apply(cases "snd (xins ! 0)",simp_all)
+    subgoal for x51
+      apply(unfold exec_push_def exec_pop_def exec_ret_def  Let_def eval_alu_def  eval_reg_def) 
+      apply(split if_splits,simp_all)
+      apply(cases " prog ! unat pc ",simp_all)
+      subgoal for x91 apply(split if_splits,simp_all)
+        using store_load_consistency
+        apply(cases "storev M64 m1 (rs1 SP - u64_of_memory_chunk M64) (Vlong (rs1 RAX))",simp_all)
+        apply(cases "loadv M64 m5 (rs5 SP)", simp_all)
+    subgoal for a apply(cases a,simp_all)
+      subgoal for x5 
+        apply(cases M64,simp_all)
+       by auto
+      done
+    done
+  done
   done
 
-
-lemma mulq_subgoal_rr_aux1:
-  assumes a0:"xins = [Pmovq_rr (bpf_to_x64_reg src) R11, Ppushl_r RDX, Pmulq_r R11, Ppopl RDX]" and
-   a1:"Next spc' reg' xm' = interp3 xins (Next spc reg xm)" and
-  a2:"(bpf_to_x64_reg dst) = RAX " and
-  a3:"bins = BPF_ALU64 BPF_MUL dst (SOReg src)" and
-  a4:"prog!(unat pc) = bins" and
-  a5:"sbpf_step prog (SBPF_OK pc rs m) = (SBPF_OK pc' rs' m')" and
-  a6:"reg (bpf_to_x64_reg dst) = rs dst" and
-  a7:"reg (bpf_to_x64_reg src) = rs src" 
-shows"reg' (bpf_to_x64_reg dst) = (rs' dst)"
+lemma mulq_subgoal_rr_aux1_3:
+  assumes a0:"xins = [(3,Pmovq_rr R11 (bpf_to_x64_reg src)), (1,Ppushl_r RAX), (3,Pmovq_rr RAX RDX), (3,Pmulq_r R11), (3,Pmovq_rr RDX RAX), (1,Ppopl RAX)]" and
+  a1:"exec_instr (snd(xins!0)) (of_nat(fst(xins!0))) xpc xrs m   = Next xpc1 xrs1 m1" and
+  a2:"exec_instr (snd(xins!1)) (of_nat(fst(xins!1))) xpc1 xrs1 m1 = Next xpc2 xrs2 m2" and
+  a3:"exec_instr (snd(xins!2)) (of_nat(fst(xins!2))) xpc2 xrs2 m2 = Next xpc3 xrs3 m3" and
+  a4:"exec_instr (snd(xins!3)) (of_nat(fst(xins!3))) xpc3 xrs3 m3 = Next xpc4 xrs4 m4" and
+  a5:"exec_instr (snd(xins!4)) (of_nat(fst(xins!4))) xpc4 xrs4 m4 = Next xpc5 xrs5 m5" and
+  a6:"exec_instr (snd(xins!5)) (of_nat(fst(xins!5))) xpc5 xrs5 m5 = Next xpc6 xrs6 m6" 
+  shows "xrs6 RAX = xrs RAX \<and> xrs6 RSP = xrs RSP"
 proof-
-  let "?xins" = "Pmulq_r (bpf_to_x64_reg src)" 
-  have "\<exists> result sz. exec_instr ?xins sz pc reg m = result" by blast
-  then obtain result sz where b1_1:"exec_instr ?xins sz spc reg xm = result" by auto
-  have "result \<noteq> Stuck"using exec_instr_def b1_1 by auto
-  hence b1:"\<exists> pc1 reg1 m1. Next pc1 reg1 m1 = exec_instr ?xins sz spc reg xm" using b1_1
-    by (metis outcome.exhaust)
-  then obtain pc1 reg1 m1 where b1:"Next pc1 reg1 m1 = exec_instr ?xins sz spc reg xm" by auto
-  have b2:"reg1 (bpf_to_x64_reg dst) =  reg' (bpf_to_x64_reg dst)" using  mulq_subgoal_rr_aux1_1 a0 a1 a2 b1 by simp
-  have b3:"reg1 (bpf_to_x64_reg dst) =  rs' dst" using mulq_subgoal_rr_aux1_2 a2 a3 a4 a5 a6 a7 b1 by simp
-  thus ?thesis using b2 b3 by auto
+  have b1:"m1 = m" using  a0 exec_instr_def a1 by simp
+  have c1:"xrs SP = xrs1 SP" using a0 exec_instr_def a1 by auto
+  have d1:"xrs RAX = xrs1 RAX" using a0 exec_instr_def a1 by auto
+
+  have b2_1:"Next xpc2 xrs2 m2 = exec_push xpc1 1 M64 m1 xrs1 (xrs1 RAX)" using exec_instr_def exec_push_def a0 a2 by auto
+  let "?addr" = "(xrs1 SP)- (u64_of_memory_chunk M64)"
+  have b2_2:"storev M64 m1 ?addr (Vlong (xrs1 RAX)) \<noteq> None" 
+    using a0 a1 exec_push_def apply(cases "storev M64 m ?addr (Vlong (xrs1 RAX))",simp_all)
+    apply (metis (no_types, lifting) memory_chunk.simps(16) storev_def val.simps(29))    
+    subgoal for a using b1 by blast
+    done
+  have b2:"storev M64 m1 ?addr (Vlong (xrs1 RAX)) = Some m2" 
+    using b2_2 b2_1 exec_push_def
+    by(cases "storev M64 m1 ?addr (Vlong (xrs1 RAX))",simp_all)
+  have c2:"xrs2 RSP = ?addr" using b2_1 exec_push_def b2_2 b2_1
+    by(cases "storev M64 m1 ?addr (Vlong (xrs1 RAX))",simp_all) 
+  have d2:"xrs2 RAX = xrs1 RAX" using a0 exec_instr_def a2 b2_1 exec_push_def 
+    by(cases "storev M64 m1 ?addr (Vlong (xrs1 RAX))",simp_all) 
+  
+  have b3:"m2=m3" using a0 exec_instr_def a3 by simp
+  have c3:"xrs2 RSP = xrs3 RSP" using  a0 exec_instr_def a3 by auto
+
+  have b4:"m3=m4" using  a0 exec_instr_def a4 by simp
+  have c4:"xrs3 RSP = xrs4 RSP" using a0 exec_instr_def a4 by auto
+
+  have b5:"m4=m5" using a0 exec_instr_def a5 by simp
+  have c5:"xrs4 RSP = xrs5 RSP" using a0 exec_instr_def a5 by auto
+
+  have b5_1:"Next xpc6 xrs6 m6 = exec_pop xpc5 1 M64 m5 xrs5 RAX" using a6 a0 exec_instr_def by simp
+  have b5_2:"Mem.loadv M64 m5 ?addr \<noteq> None" using store_load_consistency b2 b3 b4 b5 by blast
+  have b5_3:"Mem.loadv M64 m5 ?addr = Some (Vlong (xrs1 RAX))" using b2 b3 b4 b5 store_load_consistency by auto
+  have b5:"m6 = m5 \<and> xrs6 RSP = xrs RSP" using exec_pop_def b5_2
+    apply(cases "Mem.loadv M64 m5 ?addr",simp_all) 
+     apply(cases "Vlong (xrs1 RAX)",simp_all)
+    subgoal for a x5 
+      using b5_1 b5_3 c2 c3 c4 c5 c1 by force
+    done
+  have d5:"xrs6 RAX = xrs RAX" using exec_pop_def b5_2
+    apply(cases "Mem.loadv M64 m5 ?addr",simp_all) 
+     apply(cases "Vlong (xrs1 RAX)",simp_all)
+    subgoal for a x5 
+      using b5_1 b5_3 c2 c3 c4 c5 d1 d2 by force
+    done
+  thus ?thesis using d5 b5 by simp
 qed
+
+lemma mulq_subgoal_rr_aux1_4:
+  "xins = [(3,Pmovq_rr R11 (bpf_to_x64_reg src)), (1,Ppushl_r RAX), (3,Pmovq_rr RAX RDX), (3,Pmulq_r R11), (3,Pmovq_rr RDX RAX), (1,Ppopl RAX)] \<Longrightarrow>
+    exec_instr (snd(xins!0)) (of_nat(fst(xins!0))) pc rs xm = Next pc1 rs1 m1\<and>
+    exec_instr (snd(xins!1)) (of_nat(fst(xins!1))) pc1 rs1 m1 = Next pc2 rs2 m2 \<and>
+    exec_instr (snd(xins!2)) (of_nat(fst(xins!2))) pc2 rs2 m2 = Next pc3 rs3 m3 \<and>
+    exec_instr (snd(xins!3)) (of_nat(fst(xins!3))) pc3 rs3 m3 = Next pc4 rs4 m4 \<and>
+    exec_instr (snd(xins!4)) (of_nat(fst(xins!4))) pc4 rs4 m4 = Next pc5 rs5 m5 \<and> 
+    exec_instr (snd(xins!5)) (of_nat(fst(xins!5))) pc5 rs5 m5 = Next pc6 rs6 m6 \<Longrightarrow>
+  \<forall> r. bpf_to_x64_reg r \<notin> {RDX} \<longrightarrow> rs (bpf_to_x64_reg r) = rs6 (bpf_to_x64_reg r) "
+  using mulq_subgoal_rr_aux1_3 mulq_subgoal_rr_aux1_1 reg_r11_consist reg_rsp_consist 
+  by (smt (z3) insert_iff)
 
 
 lemma mulq_subgoal_rr_aux2_1:
@@ -308,16 +357,6 @@ lemma mulq_subgoal_rr_aux2_1:
   Next pc' reg' m' = exec_instr xins sz pc reg m \<Longrightarrow>
   \<forall> r. r \<notin> {RAX, RDX} \<longrightarrow> reg' r = reg r"
   by (simp add: exec_instr_def)
-
-lemma mulq_subgoal_rr_aux2_2:"xins = Pmulq_r (bpf_to_x64_reg src) \<Longrightarrow> 
-  Next pc' reg' m' = exec_instr xins sz pc reg m \<Longrightarrow>
-  \<forall> r.  bpf_to_x64_reg r \<notin> {RAX, RDX} \<longrightarrow> reg' (bpf_to_x64_reg r) = reg (bpf_to_x64_reg r)"
-  using mulq_subgoal_rr_aux2_1 by simp
-
-lemma mulq_subgoal_rr_aux2:"xins = Pmulq_r (bpf_to_x64_reg src) \<Longrightarrow> 
-  Next pc' reg' m' = exec_instr xins sz pc reg m \<Longrightarrow>
-  \<forall> r.  r \<noteq> dst \<longrightarrow> reg' (bpf_to_x64_reg r) = reg (bpf_to_x64_reg r)"
-  using mulq_subgoal_rr_aux2_1 sorry
 
 
 lemma mulq_subgoal_rr_aux3:"bins = BPF_ALU64 BPF_MUL dst (SOReg src) \<Longrightarrow> 
@@ -345,6 +384,14 @@ proof-
 qed
 
 lemma mem_is_not_changed_by_add:"Next spc' reg' m' = exec_instr xins sz spc reg m \<Longrightarrow> xins = Paddq_rr (bpf_to_x64_reg dst) (bpf_to_x64_reg src) 
+   \<Longrightarrow> m = m'"
+  using exec_instr_def by simp
+
+lemma mem_is_not_changed_by_mov:"Next spc' reg' m' = exec_instr xins sz spc reg m \<Longrightarrow> xins = Pmovq_rr (bpf_to_x64_reg dst) (bpf_to_x64_reg src) 
+   \<Longrightarrow> m = m'"
+  using exec_instr_def by simp
+
+lemma mem_is_not_changed_by_mul:"Next spc' reg' m' = exec_instr xins sz spc reg m \<Longrightarrow> xins = Pmulq_r (bpf_to_x64_reg src) 
    \<Longrightarrow> m = m'"
   using exec_instr_def by simp
 
@@ -417,9 +464,10 @@ lemma addq_subgoal_rr_generic:
        a7:"prog!(unat pc) = bins"
   shows "match_state (SBPF_OK pc' rs' m') (Next spc' reg' xm') "
 proof -
-  have b0:"xins = Paddq_rr (bpf_to_x64_reg dst) (bpf_to_x64_reg src)" using x64_encode_decode_consistency per_jit_add_reg64_1_def a1 a3 
+    have b0:"xins = Paddq_rr (bpf_to_x64_reg dst) (bpf_to_x64_reg src)" 
+      using x64_encode_decode_consistency per_jit_add_reg64_1_def a1 a3 list_in_list_prop
     by (smt (verit, ccfv_SIG) Pair_inject map_option_eq_Some option.inject)
-    moreover have b1:"(\<forall> r. (rs r) = reg (bpf_to_x64_reg r))" using a6 spec match_state_def by simp
+    moreover have b1:"(\<forall> r. (rs r) = reg (bpf_to_x64_reg r))" using a6 spec match_state_def match_reg_def by simp
     moreover have b2:"(rs src) = reg (bpf_to_x64_reg src)" using a6 spec b1 by simp
     hence b3:"(rs' dst) = reg' (bpf_to_x64_reg dst)" using aluq_subgoal_rr_aux1 b0 b1 b2 a0 a4 a5 a7 by metis
     have b4:"\<forall> r \<noteq> dst. reg'(bpf_to_x64_reg r) = reg (bpf_to_x64_reg r)" using b0 a5 aluq_subgoal_rr_aux2 by blast
@@ -429,7 +477,7 @@ proof -
     have b8:"match_stack reg' xm'" using stack_is_not_changed_by_add a6 match_state_def a5 b0 by simp
     have b9:"match_mem m' xm'" using mem_is_not_changed mem_is_not_changed_by_add match_state_def a6
       by (metis (no_types, lifting) a4 a5 b0 outcome.simps(4) sbpf_state.simps(9))
-    thus ?thesis using b3 b7 match_state_def b8 b9 by fastforce
+    thus ?thesis using b3 b7 match_state_def b8 b9 match_reg_def by fastforce
   qed
       
 
@@ -445,9 +493,9 @@ lemma exit_subgoal_rr_generic:
      shows "match_state st' xst'"
 proof-
   have b0:"st' = SBPF_Success (rs BR0)" using a0 a4 a7 a8 by simp
-  have b1:"xins = Pret" using x64_encode_decode_consistency per_jit_exit_def a0 a1 a3
+  have b1:"xins = Pret" using x64_encode_decode_consistency per_jit_exit_def a0 a1 a3 list_in_list_prop
     by (smt (verit, ccfv_SIG) map_option_eq_Some option.inject prod.inject)
-  moreover have b2:"(\<forall> r. (rs r) = reg (bpf_to_x64_reg r))" using a6 spec match_state_def by simp
+  moreover have b2:"(\<forall> r. (rs r) = reg (bpf_to_x64_reg r))" using a6 spec match_state_def match_reg_def by simp
   moreover have b3:"(rs BR0) = reg (bpf_to_x64_reg BR0)" using a6 spec b2 by simp
   (*have b4:"Mem.loadv M64 m ((reg SP) + (u64_of_memory_chunk M64)) \<noteq> None" using match_state_def a6 match_stack_def by auto
   hence "\<exists> x. Mem.loadv M64 m ((reg SP) + (u64_of_memory_chunk M64)) = x \<and> x\<noteq> None" by simp
@@ -580,435 +628,6 @@ next
 qed
 
 
-(*lemma aux3:"jit prog = x64_prog \<Longrightarrow> x64_prog \<noteq> None \<Longrightarrow> length (the x64_prog) = length prog"
-  by (metis length_map option.sel)
-
-lemma aux4:"jit prog = x64_prog \<Longrightarrow> x64_prog \<noteq> None \<Longrightarrow> unat pc \<ge> 0 \<and> unat pc < length prog \<Longrightarrow> prog \<noteq> [] \<Longrightarrow>
-  prog!(unat pc) = bins \<Longrightarrow> (the x64_prog)!(unat pc) = l_bin 
-  \<Longrightarrow> Some l_bin = per_jit_ins bins"
-  using jit_def aux3 by (metis (no_types, lifting) list.map_comp map_equality_iff nth_map nth_mem option.collapse option.sel)
-*)
-
                                   
-lemma demo1: assumes a0:"s' = sbpf_step prog s" and
-  a1:"s = (SBPF_OK pc rs m)" and
-  a2:"s' = (SBPF_OK pc' rs' m')" and
-  a3:"xst = (Next xpc xrs xm)" and
-  a4:"match_state s xst" and
-  a5:"jitper prog = Some x64_prog" and
-  a6:"prog \<noteq> [] \<and> unat pc < length prog \<and> unat pc \<ge> 0" and
-  a7:"xpc = 0" 
-shows "\<exists> xst'. let l = (x64_prog!(unat pc)) in x64_sem (fst l) (snd (snd l)) xst = xst' \<and> 
-  match_state s' xst'"
-(* \<and> snd xst' = unat (pc+1)*)
-proof-
-  let "?bpf_ins" = "prog!(unat pc)"
-  have b0:"length prog \<noteq> 0" using a6 by blast
-  have b1:"\<exists> src dst. ?bpf_ins = BPF_ALU64 BPF_ADD dst (SOReg src) \<or> ?bpf_ins = BPF_ALU64 BPF_MUL dst (SOReg src)" using a0 a1 a2 a6 b0 aux1 by blast
-  obtain src dst where b2:"?bpf_ins = BPF_ALU64 BPF_ADD dst (SOReg src) \<or> ?bpf_ins = BPF_ALU64 BPF_MUL dst (SOReg src)" using b1 by blast
-  show ?thesis
-  proof (cases "?bpf_ins = BPF_ALU64 BPF_ADD dst (SOReg src)")
-    case True
-    let "?l_bin"= "snd (snd (the (per_jit_ins ?bpf_ins)))"
-    have c0:"?l_bin = snd (snd (the (per_jit_add_reg64_1 dst src)))" using b2 True by fastforce
-    have c1:"Some ?l_bin = x64_encode (Paddq_rr (bpf_to_x64_reg dst) (bpf_to_x64_reg src))" using per_jit_add_reg64_1_def c0 by fastforce
-    have c2:"snd (snd (x64_prog!(unat pc))) = ?l_bin" using a6 c0 a5 aux5 by metis
-    let "?st" = "x64_sem (fst (x64_prog!(unat pc))) ?l_bin xst"
-    have "x64_prog!(unat pc) = the (per_jit_ins ?bpf_ins)" using aux5 a5 a6 by blast
-    then have "x64_prog!(unat pc) = the (per_jit_add_reg64_1 dst src)" using b2 True by simp
-    then have "(fst (x64_prog!(unat pc))) = 1" using per_jit_add_reg64_1_def by simp
-    hence c3:"\<exists> size2 xins2. x64_decode 0 ?l_bin = Some (length ?l_bin, xins2) \<and> ?st = exec_instr xins2 size2 xpc xrs xm" using x64_encode_decode_consistency a3 a7 c1 by fastforce
-    obtain size2 xins2 where c4:"x64_decode 0 ?l_bin = Some (length ?l_bin, xins2) \<and> ?st = exec_instr xins2 size2 xpc xrs xm" using c3 by auto
-    have c5:"xins2 = Paddq_rr (bpf_to_x64_reg dst) (bpf_to_x64_reg src)" using Pair_inject c4 c1 option.inject x64_encode_decode_consistency by metis
-    have c6:"\<exists> xrs' xpc' xm'. ?st = Next xpc' xrs' xm'" using exec_instr_def spec c5 c4 by auto
-    obtain xrs' xpc' xm' where c7:"?st = Next xpc' xrs' xm'" using c6 by auto
-    have "match_state s' ?st" using addq_subgoal_rr_generic a0 a1 a2 c7 a4 a3 c1 per_jit_add_reg64_1_def b2 c4 True by fastforce
-    then show ?thesis using True b2 c2 by force
-  next
-    case False
-    let "?l_bin"= "snd (snd (the (per_jit_ins ?bpf_ins)))"
-    have c0:"?l_bin = snd (snd (the (per_jit_mul_reg64 dst src)))" using b2 False by fastforce
-    have c1:"Some ?l_bin = (let ins_list = case (bpf_to_x64_reg dst) of
-    RAX \<Rightarrow> [Pmovq_rr (bpf_to_x64_reg src) R11, Ppushl_r RDX, Pmulq_r R11, Ppopl RDX]|
-    RDX \<Rightarrow> [Pmovq_rr (bpf_to_x64_reg src) R11, Ppushl_r RAX, Pmovq_rr RAX RDX, Pmulq_r R11, Pmovq_rr RDX RAX, Ppopl RAX]|
-    _   \<Rightarrow> [Pmovq_rr (bpf_to_x64_reg src) R11, Ppushl_r RAX, Pmovq_rr RAX (bpf_to_x64_reg dst), Ppushl_r RDX, Pmulq_r R11, 
-            Ppopl RDX, Pmovq_rr (bpf_to_x64_reg dst) RAX, Ppopl RAX]
-  in (x64_encodes_suffix ins_list))" using per_jit_mul_reg64_def c0 sorry
-    have c2:"snd (snd (x64_prog!(unat pc))) = ?l_bin" using a6 c0 a5 aux5 by metis
-    let "?st" = "x64_sem (fst (x64_prog!(unat pc))) ?l_bin xst"
-    have "x64_prog!(unat pc) = the (per_jit_ins ?bpf_ins)" using aux5 a5 a6 by blast
-    then have "x64_prog!(unat pc) = the (per_jit_mul_reg64 dst src)" using b2 False by simp
-    then show ?thesis sorry
-  qed
-qed
-  (*let "?l_bin"= "snd (snd (the (per_jit_ins ?bpf_ins)))"
-  have c0:"?l_bin = snd (snd (the (per_jit_add_reg64_1 dst src)))" using b2 by fastforce
-  have c1:"Some ?l_bin = x64_encode (Paddq_rr (bpf_to_x64_reg dst) (bpf_to_x64_reg src))" using per_jit_add_reg64_1_def c0 by fastforce
-  have c2:"snd (snd (x64_prog!(unat pc))) = ?l_bin" using a6 c0 a5 aux5 by metis
-  let "?st" = "x64_sem (fst (x64_prog!(unat pc))) ?l_bin xst"
-  have "x64_prog!(unat pc) = the (per_jit_ins ?bpf_ins)" using aux5 a5 a6 by blast
-  then have "x64_prog!(unat pc) = the (per_jit_add_reg64_1 dst src)" using b2 by simp
-  then have "(fst (x64_prog!(unat pc))) = 1" using per_jit_add_reg64_1_def by simp
-  hence c3:"\<exists> size2 xins2. x64_decode 0 ?l_bin = Some (length ?l_bin, xins2) \<and> ?st = exec_instr xins2 size2 xpc xrs xm" using x64_encode_decode_consistency a3 a7 c1 by fastforce
-  obtain size2 xins2 where c4:"x64_decode 0 ?l_bin = Some (length ?l_bin, xins2) \<and> ?st = exec_instr xins2 size2 xpc xrs xm" using c3 by auto
-  have c5:"xins2 = Paddq_rr (bpf_to_x64_reg dst) (bpf_to_x64_reg src)" using Pair_inject c4 c1 option.inject x64_encode_decode_consistency by metis
-  have c6:"\<exists> xrs' xpc' xm'. ?st = Next xpc' xrs' xm'" using exec_instr_def spec c5 c4 by auto
-  obtain xrs' xpc' xm' where c7:"?st = Next xpc' xrs' xm'" using c6 by auto
-  have "match_state s' ?st" using addq_subgoal_rr_generic a0 a1 a2 c7 a4 a3 c1 per_jit_add_reg64_1_def b2 c4 by fastforce
-  thus ?thesis using c2 by simp
-  qed*)
-
-lemma match_s_not_stuck:"match_state s xst \<Longrightarrow> xst \<noteq> Stuck"
-  apply(cases s, simp_all)
-  apply(unfold match_state_def)
-  subgoal for x11 x12 x13 by auto
-  subgoal for x2 by auto
-  by simp
-
-(*
-lemma x64_sem1_induct:"x64_sem1 (Suc n) pc x64_prog (Next xpc xrs m) = xst' \<Longrightarrow> 
-  x64_prog!(unat pc) = (num,off,l) \<Longrightarrow>
-  x64_sem num l (Next 0 xrs1 m1) = Next xpc1 xrs1 m1 \<Longrightarrow> 
-  x64_sem1 n (pc+off) x64_prog (Next xpc1 xrs1 m1) = xst'"
-  apply(cases "x64_prog!(unat pc)",simp_all)
-  subgoal for a apply(cases "(Next 0 xrs1 m1)",simp_all)
-    subgoal for x11
-*)
-
-lemma x64_sem1_induct_aux1:"x64_sem1 (Suc n) pc x64_prog (Next xpc xrs m) = xst' \<Longrightarrow> 
-  x64_prog!(unat pc) = (num,off,l) \<Longrightarrow>
-  x64_sem num l (Next 0 xrs m) = xst1 \<Longrightarrow> 
-  x64_sem1 n (pc+off) x64_prog xst1 = xst'"
- apply(induct n arbitrary:pc x64_prog xpc xrs m xst' num off l)
- apply simp 
-  by simp
-
-lemma x64_sem1_induct_aux2:"x64_sem1 n pc x64_prog (Next xpc xrs xm) = x64_sem1 n pc x64_prog (Next 0 xrs xm)"
-proof(cases n)
-  case 0
-  then show ?thesis by simp
-next
-  case (Suc n)
-    thus ?thesis using Suc by fastforce
-qed
- 
-lemma x64_sem1_induct_aux3:"
-  xst = (Next xpc xrs m) \<Longrightarrow>
-  x64_sem1 (Suc n) pc x64_prog xst = xst' \<Longrightarrow> 
-  x64_prog!(unat pc) = (num,off,l) \<Longrightarrow>
-  x64_sem num l (Next 0 xrs m) = xst1 \<Longrightarrow> 
-  xst1 = Next xpc1 xrs1 m1 \<Longrightarrow>
-  x64_sem1 n (pc+off) x64_prog (Next 0 xrs1 m1) = xst'"
-  using x64_sem1_induct_aux2 x64_sem1_induct_aux1 by metis
-
-lemma pc_scope_aux:"\<lbrakk> sbpf_sem n prog s = s'; s = (SBPF_OK pc rs m); s' = (SBPF_OK pc' rs' m'); prog \<noteq> []; n>0\<rbrakk> \<Longrightarrow> 
-  unat pc < length prog \<and> unat pc \<ge> 0"
-  by (metis (no_types, opaque_lifting) err_is_still_err linorder_not_less not_gr_zero sbpf_sem.elims sbpf_state.simps(6) sbpf_step.simps(1))
-
-(*
-lemma num_is_1_aux:"jitper prog = Some x64_prog \<Longrightarrow> prog \<noteq> [] \<and> unat pc < length prog \<and> 0 \<le> unat pc \<Longrightarrow> 
-  fst (x64_prog!(unat pc)) = 1"
-proof (induction prog arbitrary:x64_prog pc)
-  case Nil
-  then show ?case by blast
-next
-  case (Cons a prog)
-  then show ?case 
-  proof-
-    have a0:"unat pc = 0 \<or> unat pc \<ge> 1" by auto
-    have b0:"\<exists> x. per_jit_ins a = Some x" using Cons by (cases "per_jit_ins a"; auto)
-    obtain x where b1:"per_jit_ins a = Some x" using b0 by auto
-    then have b2:"\<exists> res. jitper prog = Some res" using Cons(1) apply (cases "jitper prog"; auto) 
-      using Cons.prems(1) by simp
-    obtain res where b3:"jitper prog = Some res"  using b2 by blast
-    have b4:"x64_prog = x # res" using Cons(1) b3 b1 Cons by force
-    show ?thesis
-    proof (cases "unat pc = 0")
-      case True
-      have b5:"unat pc = 0" using True a0 by simp
-      have b6:"fst (the (per_jit_ins a)) = 1"  
-        apply(cases "per_jit_ins a",simp_all)
-        using b1 apply fastforce
-        subgoal for aa apply(cases a,simp_all)
-          subgoal for x91 x92 x93
-            apply(cases x91, simp_all)
-            apply(cases x93,simp_all)
-            subgoal for x2 
-              apply(unfold per_jit_add_reg64_1_def Let_def,simp_all) 
-              using b5 by auto
-            done
-          apply(unfold per_jit_exit_def,simp_all)
-          using b5 by auto
-        done
-      have b7:"the (per_jit_ins a) = x64_prog!(unat pc)" using b5 b1 b4 by auto
-      then show ?thesis using b6 b7 by auto
-    next
-      case False
-      have c0:" Some (x # res) = Some x64_prog" using b4 by blast
-      have c1:"unat pc \<ge> 1" using a0 False by blast
-      let "?pc'" = "unat pc -1"
-      have c2:"0 \<le> ?pc' \<and> ?pc' < length prog \<and> prog \<noteq> []" using Cons 
-        by (metis False One_nat_def c1 length_Cons less_diff_conv2 less_one list.size(3) list.size(4) zero_le)
-      hence "fst (x64_prog ! unat pc) = 1" using c2 Cons False b3
-        by (metis (no_types, lifting) b4 nth_Cons' unat_minus_one unsigned_eq_0_iff)
-      then show ?thesis by blast
-    qed
-  qed
-qed
-*)
-
-lemma corr_pc_aux1:"jitper prog = Some x64_prog \<Longrightarrow> 
-  prog \<noteq> [] \<and> unat pc \<ge> 0 \<and> unat pc < length prog \<Longrightarrow>
-  (num,off,l) = x64_prog!(unat pc) \<Longrightarrow>
-  off=1"
-proof (induction prog arbitrary: x64_prog pc num off l)
-  case Nil
-  then show ?case by simp
-next
-  case (Cons a prog)
-  then show ?case
-  proof-
-    have a0:"unat pc = 0 \<or> unat pc \<ge> 1" by auto
-    show ?thesis
-    proof (cases "unat pc = 0")
-      case True
-      have b0_1:"unat pc = 0" using True a0 by simp
-      have b0:"\<exists> x. per_jit_ins a = Some x" using Cons by (cases "per_jit_ins a"; auto)
-      obtain x where b1:"per_jit_ins a = Some x" using b0 by auto
-      have b1_1:"(num,off,l) = x" using b0_1 b1 True Cons
-        by (smt (verit) jitper.simps(2) nth_Cons_0 old.prod.case option.case_eq_if option.discI option.sel prod_cases3)
-      have bn:"off = 1" 
-        using b1 apply(cases "per_jit_ins a", simp_all) 
-        subgoal for aa 
-         apply(cases a,simp_all)
-        subgoal for x91 x92 x93
-          apply(cases x91,simp_all)
-          apply(cases x93,simp_all)
-          subgoal for x1 using b1 b1_1 per_jit_add_reg64_1_def Let_def by auto
-          apply(cases x93,simp_all) 
-          subgoal for x2 using b1 b1_1 per_jit_mul_reg64_def Let_def by (smt (verit) map_option_eq_Some prod.inject)
-          done
-        apply(unfold per_jit_exit_def Let_def, simp_all) using b1 b1_1 by blast
-      done
-      then show ?thesis using bn by blast
-    next
-      case False
-      have "\<exists> res. jitper prog = Some res" using Cons 
-        apply (cases "jitper prog"; simp_all) 
-        apply(cases a, simp_all) 
-        subgoal for x91 x92 x93 apply(cases x91,simp_all) 
-          apply(cases x93,simp_all)
-          subgoal for x2 apply(cases "per_jit_add_reg64_1 x92 x2",simp_all) 
-            done 
-          apply(cases x93,simp_all) 
-          subgoal for x2 apply(cases "per_jit_mul_reg64 x92 x2",simp_all) 
-            done
-          done
-        apply(unfold per_jit_exit_def) 
-        apply(cases per_jit_exit,simp_all) 
-        done
-      then obtain res where b0:"jitper prog = Some res" by auto
-      have b1:"\<exists> x. per_jit_ins a = Some x" using Cons by (cases "per_jit_ins a"; auto)
-      obtain x where b2:"per_jit_ins a = Some x" using b1 by auto
-      have c0:" Some (x # res) = Some x64_prog" using b0 b2 Cons by auto
-      have c1:"unat pc \<ge> 1" using a0 False by blast
-      have c2:"x64_prog ! unat pc = (num,off,l)" using c0 Cons by simp
-      let "?pc'" = "unat pc -1"
-      have c3:"(num,off,l) = res! ?pc'" using c0 False c2 by auto
-      have c4:"0 \<le> ?pc' \<and> ?pc' < length prog \<and> prog \<noteq> [] " using Cons c0 c1 by auto
-      have c5:"off=1" using c3 c4 
-        by (metis Cons.IH False b0 unat_minus_one unsigned_eq_0_iff)
-      then show ?thesis by blast
-    qed
-  qed
-qed
-
-
-lemma corr_pc_aux2:
-  "jitper prog = Some x64_prog \<Longrightarrow> prog \<noteq> [] \<and> unat pc \<ge> 0 \<and> unat pc < length prog \<Longrightarrow>
-  s =  SBPF_OK pc rs m \<Longrightarrow>
-  s' = sbpf_step prog s \<Longrightarrow> s' = SBPF_OK pc' rs' m' \<Longrightarrow> 
-  (num,off,l) = x64_prog!(unat pc) \<Longrightarrow>
-  pc' = pc+off"
-proof-
-  assume assm0:"s' = sbpf_step prog s"  and
-         assm1:"s' = SBPF_OK pc' rs' m'" and
-         assm2:"jitper prog = Some x64_prog" and
-         assm3:"prog \<noteq> [] \<and> unat pc \<ge> 0 \<and> unat pc < length prog" and
-         assm4:"s = SBPF_OK pc rs m" and
-         assm5:"(num,off,l) = x64_prog!(unat pc)"
-  have "\<exists> src dst. prog!(unat pc) \<in> {BPF_ALU64 BPF_ADD dst (SOReg src), BPF_ALU64 BPF_MUL dst (SOReg src), BPF_EXIT}" 
-    using assm0 assm1 assm3 assm4 aux2 length_0_conv sbpf_state.simps(6) by (smt (verit, del_insts) insert_commute)
-  then obtain src dst where c0:"prog!(unat pc) \<in> {BPF_ALU64 BPF_ADD dst (SOReg src), BPF_ALU64 BPF_MUL dst (SOReg src), BPF_EXIT}" by blast
-  have c1:"pc' = pc+1" using c0 assm0 assm1 apply(cases "prog!(unat pc)",simp_all)
-    prefer 2 using assm4 assm3 apply simp
-    subgoal for x91 x92 x93 apply(erule disjE)
-      using assm4 assm3 apply (smt (verit) binop.simps(133) bpf_instruction.simps(369) option.case_eq_if sbpf_state.inject(1) sbpf_state.simps(6) sbpf_step.elims)
-      using assm4 assm3 option.case_eq_if sbpf_step.elims sorry
-    done
-  have "off=1" 
-    using assm2 assm3 assm5 corr_pc_aux1 by blast
-  thus ?thesis using c1 by simp
-qed
-  (*have "x64_prog!(unat pc) = the (per_jit_ins (prog!(unat pc)))" using aux5 assm2 assm3 assm5 by blast
-  hence c2:"x64_prog!(unat pc) = the (per_jit_add_reg64_1 dst src) \<or> x64_prog!(unat pc) = the per_jit_exit" using c0 by auto
-  hence c3:"off = (fst(snd(the (per_jit_add_reg64_1 dst src)))) \<or> off = (fst(snd(the (per_jit_exit))))" using assm5 by (metis split_pairs)
-  thus ?thesis
-  proof(cases "off = (fst(snd(the (per_jit_exit))))")
-    case True
-    have "off = 1" using per_jit_add_reg64_1_def True by auto
-    then show ?thesis using c1 by simp
-  next
-    case True
-    have "off = (fst(snd(the (per_jit_exit))))" using True c3 by blast
-    hence "off = 1" using per_jit_exit_def Let_def try
-    then show ?thesis using c1 by simp
-  qed                                                   
-qed*)
-
-lemma demo2_aux:
-  "\<lbrakk> sbpf_sem n prog s = s';
-   s = (SBPF_OK pc rs m);
-   s' = (SBPF_OK pc' rs' m');
-   xst = (Next xpc xrs xm);
-   match_state s xst;
-   jitper prog = Some x64_prog;
-   prog \<noteq> [];
-   xpc = 0;
-   x64_sem1 n pc x64_prog xst = xst' \<rbrakk> \<Longrightarrow>
-   match_state s' xst'"
-(* \<exists> xst'. x64_sem1 n pc x64_prog xst = xst' \<and> match_state s' xst'"*)
-proof (induction n arbitrary: prog s s' pc rs m pc' rs' m' xst' xst xpc xrs xm x64_prog xst')
-  case 0
-  then show ?case
-    by simp
-next
-  case (Suc n)
-  assume 
-       assm1: "sbpf_sem (Suc n) prog s = s'" and
-       assm2:"s = SBPF_OK pc rs m" and
-       assm3:"s' = SBPF_OK pc' rs' m'" and
-       assm4:"xst = Next xpc xrs xm" and
-       assm5:"match_state s xst" and
-       assm6:"jitper prog = Some x64_prog" and
-       assm7:"prog \<noteq> [] " and
-       assm8:"xpc = 0" and
-       assm9:"x64_sem1 (Suc n) pc x64_prog xst = xst'"
-  then obtain s1 where s1_eq: "s1 = sbpf_step prog s" by simp
-  have n_step_def:"sbpf_sem n prog s1 = s'" using s1_eq assm1 sbpf_sem_induct
-    by (metis sbpf_sem.simps(2))
-  have a0:"unat pc < length prog \<and> unat pc \<ge> 0" using assm1 assm3 
-    using Suc.prems(2) assm7 pc_scope_aux by blast
-  moreover have a1:"\<exists> pc1 rs1 m1. s1 = (SBPF_OK pc1 rs1 m1)"
-    by (metis Suc.prems(3) bot_nat_0.not_eq_extremum intermediate_step_is_ok n_step_def sbpf_sem.simps(1) sbpf_state.simps(6))
-  obtain pc1 rs1 m1 where a2:"s1 = (SBPF_OK pc1 rs1 m1)" using a1 by auto
-  have a3:"m1 = m" using mem_is_not_changed s1_eq assm2 a2 by blast
-  let "?num" = "(fst(x64_prog!(unat pc)))"
-  have "\<exists> xst1. x64_sem (fst(x64_prog!(unat pc))) (snd (snd ((x64_prog!(unat pc)))))(Next xpc xrs xm) = xst1 \<and> match_state s1 xst1"
-    using s1_eq assm2 a2 assm4 assm5 assm6 assm7 assm8 assm8 demo1 by (metis (mono_tags, lifting) calculation)
-  then obtain xst1 where a4:"x64_sem ?num (snd (snd ((x64_prog!(unat pc)))))(Next 0 xrs xm) = xst1 \<and> match_state s1 xst1" using assm8 by auto
-  hence a4_1:"x64_sem ?num (snd (snd ((x64_prog!(unat pc)))))(Next 0 xrs xm) = xst1" by auto
-  have an:"\<exists> xpc1 xrs1 xm1. xst1 = Next xpc1 xrs1 xm1" using a4 by (metis match_s_not_stuck outcome.exhaust)
-  then obtain xpc1 xrs1 xm1 where a10:"xst1 = Next xpc1 xrs1 xm1" by auto
-  let "?xst1" = "Next 0 xrs1 xm1"
-  have a5:"match_state s1 ?xst1" using an match_state_def
-    using a10 a2 a4 by fastforce
-  have "\<exists> num off l. x64_prog!(unat pc) = (num,off,l)" by (metis split_pairs)
-  then obtain num off l where a6:"x64_prog!(unat pc) = (num,off,l)" by auto
-  have a7:"l = (snd (snd ((x64_prog!(unat pc)))))" using a6 by simp
-  let "?pc" = "pc+off"
-  have a9:"x64_sem1 n ?pc x64_prog ?xst1 = xst'" using x64_sem1_induct_aux3 assm4 assm9 a7 a6 a4_1 a10 by (metis fst_conv)
-  have a13:"?pc = pc1" using corr_pc_aux2 assm6 a0 s1_eq a6 a2 assm7 assm2 by auto
-  from Suc.IH have " sbpf_sem n prog s = s' \<Longrightarrow>
-           s = SBPF_OK pc rs m \<Longrightarrow>
-           s' = SBPF_OK pc' rs' m' \<Longrightarrow>
-           xst = Next xpc xrs xm \<Longrightarrow>
-           match_state s xst \<Longrightarrow>
-           jitper prog = Some x64_prog \<Longrightarrow>
-           prog \<noteq> [] \<and> unat pc < length prog \<and> 0 \<le> unat pc \<Longrightarrow> 
-           xpc = 0 \<Longrightarrow> 
-           x64_sem1 n pc x64_prog xst = xst' \<Longrightarrow> 
-           match_state s' xst'" by blast
-  have "x64_sem1 n pc1 x64_prog (Next 0 xrs1 xm1) = xst' \<and> match_state s' xst'" using n_step_def a2 assm3 a10 a5 assm6 assm7 assm8 a9 Suc a13 by blast
-  hence an:"match_state s' xst'" by blast
-  then show ?case using an by auto
-qed
-(*
-lemma demo2_aux:
-  "\<lbrakk> sbpf_sem n prog s = s';
-   s = (SBPF_OK pc rs m);
-   s' = (SBPF_OK pc' rs' m');
-   xst = (Next xpc xrs xm);
-   match_state s xst;
-   jitper prog = Some x64_prog;
-   prog \<noteq> [] \<and> unat pc < length prog \<and> unat pc \<ge> 0;
-   xpc = 0;
-   x64_sem1 n pc x64_prog xst = xst' \<rbrakk> \<Longrightarrow>
-   match_state s' xst'"
-(* \<exists> xst'. x64_sem1 n pc x64_prog xst = xst' \<and> match_state s' xst'"*)
-proof (induction n arbitrary: prog s s' pc rs m pc' rs' m' xst' xst xpc xrs xm x64_prog xst')
-  case 0
-  then show ?case
-    by simp
-next
-  case (Suc n)
-  assume assm1: "sbpf_sem (Suc n) prog s = s'" and
-       assm2:"s = SBPF_OK pc rs m" and
-       assm3:"s' = SBPF_OK pc' rs' m'" and
-       assm4:"xst = Next xpc xrs xm" and
-       assm5:"match_state s xst" and
-       assm6:"jitper prog = Some x64_prog" and
-       assm7:"prog \<noteq> [] \<and> unat pc < length prog \<and> 0 \<le> unat pc " and
-       assm8:"xpc = 0" and
-       assm9:"x64_sem1 (Suc n) pc x64_prog xst = xst'"
-  then obtain s1 where s1_eq: "s' = sbpf_step prog s1" 
-    by (metis add_Suc_right sbpf_sem.simps(1) sbpf_sem.simps(2) sbpf_sem_induct)
-  from Suc have s'_def:"sbpf_sem (Suc n) prog s = s'" by blast
-  have one_step_def:"\<exists> s1. sbpf_sem n prog s = s1 \<and> sbpf_step prog s1 = s'" using s1_eq s'_def sbpf_sem_induct
-    by (metis add_Suc_right sbpf_sem.simps(1) sbpf_sem.simps(2))
-  obtain s1 where get_s1:"sbpf_sem n prog s = s1 \<and> sbpf_step prog s1 = s'" using one_step_def by simp
-  have a1:"s1 = sbpf_sem n prog s" using one_step_def s1_eq using get_s1 by force
-  have a3:"\<exists> pc1 rs1 m1. s1 = (SBPF_OK pc1 rs1 m1)" 
-    by (smt (verit) Suc.prems(3) get_s1 sbpf_state.simps(6) sbpf_step.elims)
-  obtain pc1 rs1 m1 where a6:"s1 = (SBPF_OK pc1 rs1 m1)" using a3 by auto
-  moreover have "m1 = m'" using mem_is_not_changed Suc.prems(3) calculation get_s1 by blast
-  hence a4:"s1 = (SBPF_OK pc1 rs1 m')" using calculation by blast
-  have "\<exists> xst1. x64_sem1 n pc x64_prog xst = xst1" by blast
-  (*have "\<exists> xst1. x64_sem1 n pc x64_prog xst = xst1 \<and> x64_sem 1 (snd (snd ((x64_prog!(unat pc1))))) xst1 = xst'" sorry*)
-  then obtain xst1 where a2:"x64_sem1 n pc x64_prog xst = xst1" using a4 by auto
-  from Suc.IH have "sbpf_sem n prog s = s' \<Longrightarrow>
-           s = SBPF_OK pc rs m \<Longrightarrow>
-           s' = SBPF_OK pc' rs' m' \<Longrightarrow>
-           xst = Next xpc xrs m \<Longrightarrow>
-           match_state s xst \<Longrightarrow>
-           jitper prog = Some x64_prog \<Longrightarrow>
-           prog \<noteq> [] \<and> unat pc < length prog \<and> 0 \<le> unat pc \<Longrightarrow> xpc = 0 \<Longrightarrow> x64_sem1 n pc x64_prog xst = xst' \<Longrightarrow> 
-           match_state s' xst'" by blast
-  from Suc have a5:"match_state s1 xst1" using a1 assm2 a4 assm4 assm5 assm6 assm7 assm8 a2 by blast
-  have b0:"\<exists> xpc1 xrs1 m2. xst1 = (Next xpc1 xrs1 m2)" using match_s_not_stuck a5 by (meson outcome.exhaust)
-  obtain xpc1 xrs1 m2 where b0:"xst1 = (Next xpc1 xrs1 m2)" using b0 by auto
-  (*moreover have "m2 = m" using a4 a5 calculation(2) match_state_def mem_is_not_changed2 sorry*)
-  have b4:"unat pc1 < length prog \<and> unat pc1 \<ge> 0" 
-    by (metis (no_types, lifting) a4 assm3 get_s1 linorder_not_less sbpf_state.simps(6) sbpf_step.simps(1))
-  have b6:"\<exists> xst2. x64_sem 1 (snd (snd ((x64_prog!(unat pc1)))))(Next 0 xrs1 m2) = xst2 \<and> match_state s' xst2" 
-    using s1_eq a4 assm3 b0 a5 assm6 assm7 b0 demo1 b4 Suc.prems(6) get_s1 
-    by (smt (verit, ccfv_SIG) match_state_def outcome.simps(4) sbpf_state.case(1))
-  obtain xst2 where "x64_sem 1 (snd (snd ((x64_prog!(unat pc1))))) (Next 0 xrs1 m2) = xst2 \<and> match_state s' xst2" using b6 by auto
-  moreover have "xst2 = xst'" using x64_sem1_induct 
-    using a2 assm9 calculation(2) b0 sorry
-  then show ?case using calculation(2) by fastforce
-qed
-*)
-lemma demo2:
-  "\<lbrakk> sbpf_sem n prog s = s';
-   s = (SBPF_OK pc rs m);
-   s' = (SBPF_OK pc' rs' m);
-   xst = (Next xpc xrs m);
-   match_state s xst;
-   jitper prog = Some x64_prog;
-   prog \<noteq> [] \<and> unat pc < length prog \<and> unat pc \<ge> 0;
-   xpc = 0 \<rbrakk> \<Longrightarrow>
-   \<exists> xst'. x64_sem1 n pc x64_prog xst = xst' \<and> match_state s' xst'"
-  using demo2_aux by blast
 
 end
