theory/x64Assembler.thy
@@ -2,7 +2,7 @@ theory x64Assembler
   imports Main rBPFCommType rBPFSyntax x64Syntax x86CommType
 
 begin
-fun x64_encode :: "instruction \<Rightarrow> x64_bin option" where
+fun x64_encode :: "instruction \<Rightarrow> x64_bin" where
 "x64_encode ins = (
 case ins of
 Paddq_rr rd r1 \<Rightarrow>
@@ -14,9 +14,9 @@ Paddq_rr rd r1 \<Rightarrow>
       ) in
     let (op:: u8) = 0x01 in
     let (rop::u8) = construct_modsib_to_u8 0b11 (u8_of_ireg r1) (u8_of_ireg rd) in
-      Some [ rex, op, rop ] |
+     [ rex, op, rop ] |
   Pret \<Rightarrow>
-    Some [0xc3] |
+    [0xc3] |
   \<comment> \<open> P2884 `MUL RAX with qwordregister (to RDX:RAX)` -> ` 0100 100B : 1111 0111 : 11 100 qowrdreg` \<close>
   Pmulq_r r1 \<Rightarrow>
     let (rex:: u8) = (construct_rex_to_u8  \<comment> \<open> `100B` \<close>
@@ -27,7 +27,7 @@ Paddq_rr rd r1 \<Rightarrow>
       ) in
     let (op:: u8) = 0xf7 in
     let (rop::u8) = construct_modsib_to_u8 0b11 0b100 (u8_of_ireg r1) in
-      Some [ rex, op, rop] |
+      [ rex, op, rop] |
   \<comment> \<open> P2882 `MOV qwordregister1 to qwordregister2` -> `0100 1R0B : 1000 1001 : 11 reg1 reg2` \<close>
   Pmovq_rr rd r1 \<Rightarrow>
     let (rex:: u8) = (construct_rex_to_u8  \<comment> \<open> `1R0B` \<close>
@@ -38,7 +38,77 @@ Paddq_rr rd r1 \<Rightarrow>
       ) in
     let (op:: u8) = 0x89 in
     let (rop::u8) = construct_modsib_to_u8 0b11 (u8_of_ireg r1) (u8_of_ireg rd) in
-      Some [ rex, op, rop ] |
+       [ rex, op, rop ] |
+  \<comment> \<open> P2885 `PUSH: qwordregister (alternate encoding)`   -> ` 0100 W00BS : 0101 0 reg64` \<close>
+  Ppushl_r  r1 \<Rightarrow>
+    let (rex::u8) = (construct_rex_to_u8    \<comment> \<open> `000B` \<close>
+      False \<comment> \<open> W \<close>
+      False \<comment> \<open> R \<close>
+      False \<comment> \<open> X \<close>
+      (and (u8_of_ireg r1) 0b1000 \<noteq> 0) \<comment> \<open> B \<close>
+      ) in
+    let (op::u8) = bitfield_insert_u8 0 3 0x50 (u8_of_ireg r1) in
+      if rex = 0x40 then
+         [op]
+      else 
+        [rex, op] |
+  \<comment> \<open> P2885 `POP: qwordregister (alternate encoding)`   -> ` 0100 W00B : 0101 1 reg64 ` \<close>
+  Ppopl rd \<Rightarrow>
+    let (rex::u8) = (construct_rex_to_u8    \<comment> \<open> `000B` \<close>
+      False \<comment> \<open> W \<close>
+      False \<comment> \<open> R \<close>
+      False \<comment> \<open> X \<close>
+      (and (u8_of_ireg rd) 0b1000 \<noteq> 0) \<comment> \<open> B \<close>
+      ) in
+    let (op::u8) = bitfield_insert_u8 0 3 0x58 (u8_of_ireg rd) in
+      if rex = 0x40 then
+         [op]
+      else 
+          [rex, op] )"
+
+
+fun list_in_list :: "'a list \<Rightarrow> nat \<Rightarrow> 'a list \<Rightarrow> bool" where
+"list_in_list [] _ _ = True" |
+"list_in_list (h#t) n l = (h = l!n \<and> list_in_list t (Suc n) l)"
+
+
+(*fun x64_encode :: "instruction \<Rightarrow> (nat \<times> x64_bin) option" where
+"x64_encode ins = (
+case ins of
+Paddq_rr rd r1 \<Rightarrow>
+    let (rex:: u8) = (construct_rex_to_u8  \<comment> \<open> `1R0B` \<close>
+      True \<comment> \<open> W \<close>
+      (and (u8_of_ireg r1) 0b1000 \<noteq> 0) \<comment> \<open> R \<close>
+      False \<comment> \<open> X \<close>
+      (and (u8_of_ireg rd) 0b1000 \<noteq> 0) \<comment> \<open> B \<close>
+      ) in
+    let (op:: u8) = 0x01 in
+    let (rop::u8) = construct_modsib_to_u8 0b11 (u8_of_ireg r1) (u8_of_ireg rd) in
+      Some (3, [ rex, op, rop ]) |
+  Pret \<Rightarrow>
+    Some (1,[0xc3]) |
+  \<comment> \<open> P2884 `MUL RAX with qwordregister (to RDX:RAX)` -> ` 0100 100B : 1111 0111 : 11 100 qowrdreg` \<close>
+  Pmulq_r r1 \<Rightarrow>
+    let (rex:: u8) = (construct_rex_to_u8  \<comment> \<open> `100B` \<close>
+      True \<comment> \<open> W \<close>
+      False \<comment> \<open> R \<close>
+      False \<comment> \<open> X \<close>
+      (and (u8_of_ireg r1) 0b1000 \<noteq> 0) \<comment> \<open> B \<close>
+      ) in
+    let (op:: u8) = 0xf7 in
+    let (rop::u8) = construct_modsib_to_u8 0b11 0b100 (u8_of_ireg r1) in
+      Some (3,[ rex, op, rop]) |
+  \<comment> \<open> P2882 `MOV qwordregister1 to qwordregister2` -> `0100 1R0B : 1000 1001 : 11 reg1 reg2` \<close>
+  Pmovq_rr rd r1 \<Rightarrow>
+    let (rex:: u8) = (construct_rex_to_u8  \<comment> \<open> `1R0B` \<close>
+      True \<comment> \<open> W \<close>
+      (and (u8_of_ireg r1) 0b1000 \<noteq> 0) \<comment> \<open> R \<close>
+      False \<comment> \<open> X \<close>
+      (and (u8_of_ireg rd) 0b1000 \<noteq> 0) \<comment> \<open> B \<close>
+      ) in
+    let (op:: u8) = 0x89 in
+    let (rop::u8) = construct_modsib_to_u8 0b11 (u8_of_ireg r1) (u8_of_ireg rd) in
+      Some (3,[ rex, op, rop ]) |
   \<comment> \<open> P2885 `PUSH: qwordregister (alternate encoding)`   -> ` 0100 W00BS : 0101 0 reg64` \<close>
   Ppushl_r  r1 \<Rightarrow>
     let (rex::u8) = (construct_rex_to_u8    \<comment> \<open> `000B` \<close>
@@ -65,7 +135,7 @@ Paddq_rr rd r1 \<Rightarrow>
         Some [op]
       else 
         Some [rex, op] )"
-
+*)
 
 value "x64_encode (Paddq_rr RAX RBX)"
 value "x64_encode (Pret)"
@@ -81,109 +151,63 @@ value "construct_rex_to_u8  \<comment> \<open> `1R0B` \<close>
 "list_in_list [] _ _ = True" |
 "list_in_list (h#t) n l = (h = l!n \<and> list_in_list t (Suc n) l)"*)
 
-fun x64_encodes_aux :: "instruction list \<Rightarrow> x64_bin option list" where
-"x64_encodes_aux [] = [None]" |
-"x64_encodes_aux (h#t) = (let ins' = x64_encode h in 
-                        (case ins' of None \<Rightarrow> [None] |
-                                      Some v \<Rightarrow> [Some v] @ x64_encodes_aux t))"
-
-definition x64_encodes:: "instruction list \<Rightarrow> x64_bin list option" where
-"x64_encodes xs = (let x = x64_encodes_aux xs in if x = [None] then None  
-                   else Some (map Option.the (butlast x)))"
-
 primrec flat :: "'a list list => 'a list" where
   "flat [] = []" |
   "flat (x # xs) = x @ flat xs"
-
-definition x64_encodes_suffix:: "instruction list \<Rightarrow> x64_bin option" where
-"x64_encodes_suffix xs = (let l = x64_encodes xs in (if l = None then None else Some (flat (Option.the l))))"
-
 
 
 (*primrec flat2 :: "'a list list option=> 'a list option" where
   "flat2 None = None" |
   "flat2 res = x @ flat xs"*)
 
-fun x64_encodes1 :: "instruction list \<Rightarrow> x64_bin list option" where
-  "x64_encodes1 [] = Some []" |
-  "x64_encodes1 (h#xs) = (case x64_encode h of 
-                            None \<Rightarrow> None |
-                            Some x \<Rightarrow> 
-                              (case x64_encodes1 xs of
-                                None \<Rightarrow> None |
-                                Some res \<Rightarrow> Some (x#res)))"
+fun x64_encodes1 :: "instruction list \<Rightarrow> x64_bin list" where
+  "x64_encodes1 [] = []" |
+  "x64_encodes1 (h#xs) = ((x64_encode h)# (x64_encodes1 xs))"
 
-definition x64_encodes2 :: "instruction list \<Rightarrow> x64_bin option" where
-"x64_encodes2 xs = (let x = (x64_encodes1 xs) in 
-    case x of None \<Rightarrow> None |
-              Some x \<Rightarrow> Some (flat x))"
+definition x64_encodes2 :: "instruction list \<Rightarrow> x64_bin" where
+"x64_encodes2 xs = (let x = (x64_encodes1 xs) in (flat x))"
 
-lemma x64_encodes1_induct:"x64_encodes1 insns = Some res \<Longrightarrow>
+lemma x64_encodes1_induct:"x64_encodes1 insns = res \<Longrightarrow>
   insns = (h#xs) \<Longrightarrow>
-  (x64_encode h) = Some res1 \<Longrightarrow> 
-  (x64_encodes1 xs) = Some res2 \<Longrightarrow>
+  (x64_encode h) = res1 \<Longrightarrow> 
+  (x64_encodes1 xs) =res2 \<Longrightarrow>
   res = res1#res2"
   apply(induction insns arbitrary: res h xs res1 res2)
    apply simp
   subgoal for a insns res h xs res1 res2 by simp
   done
 
-
-lemma x64_encodes2_equiv:"Some res = x64_encode ins \<Longrightarrow>
-  Some resn = x64_encodes2 [ins] \<Longrightarrow>
+lemma x64_encodes2_equiv:"res = x64_encode ins \<Longrightarrow>
+  resn = x64_encodes2 [ins] \<Longrightarrow>
   res = resn"
   using x64_encodes2_def by (metis (mono_tags) append.right_neutral flat.simps(1) flat.simps(2) option.sel option.simps(5) x64_encodes1.simps(1) x64_encodes1.simps(2))
 
 lemma x64_encodes2_induct:
   assumes 
-  a1:"x64_encodes2 insns = Some res" and
+  a1:"x64_encodes2 insns = res" and
   a2:"insns = (h#xs)" and
-  a3:"(x64_encode h) = Some res1" and
-  a4:"(x64_encodes2 xs) = Some res2"
+  a3:"(x64_encode h) = res1" and
+  a4:"(x64_encodes2 xs) = res2"
 shows "res = res1@res2"
- (* using x64_encodes1_induct x64_encodes2_def apply(cases "(x64_encodes1 xs)",simp_all*)
 proof-
-  have "\<exists>result. result = (x64_encodes1 xs)" by blast
-  then obtain result where b0:"result = (x64_encodes1 xs)" by auto
-  hence b1:"res2 = flat (the result)" using x64_encodes2_def a4 by(cases "x64_encodes1 xs",simp_all)
-  hence "\<exists> res2'. result = Some res2'" using a4 
-    using b0 option.collapse x64_encodes2_def by fastforce
-  then obtain res2' where b2:"result = Some res2'" by auto
+  have "\<exists>res2'. res2' = (x64_encodes1 xs)" by blast
+  then obtain res2' where b0:"res2' = (x64_encodes1 xs)" by auto
+  hence b1:"res2 = flat res2'" using x64_encodes2_def a4 by simp
   hence b3:"res2 = flat res2'" using b1 by simp
   hence "\<exists> res'. res' = res1#res2'" by simp
   then obtain res' where b4:"res' = res1#res2'" by auto
-  have "flat res' = res" using b4 b2 a1 a2 a3 b0 x64_encodes2_def by auto
+  have "flat res' = res" using b4 a1 a2 a3 b0 x64_encodes2_def by simp
   thus ?thesis by (simp add: b4 b3)
 qed
 
-(*
 
-
-fun x64_encodes_func :: "instruction list \<Rightarrow> x64_bin option" where
-"x64_encodes_func [] = None"|
-"x64_encodes_func (h#t) = (let ins' = x64_encode h in 
-                        (case ins' of None \<Rightarrow> None |
-                                      Some v \<Rightarrow> Some (v @ the (x64_encodes_func t))))"
-definition x64_encodes_func_suffix:: "instruction list \<Rightarrow> x64_bin option" where
-"x64_encodes_func_suffix xs = (let l = x64_encodes_func xs in (if l = None then None else Some (butlast(the l))))"
-
-
-value "x64_encodes_func [Pmovq_rr src dst,Pmovq_rr src dst]"
-value "x64_encodes_func_suffix [Pmovq_rr src dst,Pmovq_rr src dst]"
-
-lemma "x64_encodes_suffix xs = x64_encodes_func_suffix xs"
-  apply(unfold x64_encodes_suffix_def x64_encodes_func_suffix_def Let_def x64_encodes_def)
-  apply(split if_splits,simp_all)
-  sorry
-
-*)
 value "x64_encode (Pmovq_rr src dst)"
-value "x64_encodes [Pmovq_rr src dst, Pmovq_rr src dst]"
 value "x64_encodes1 [Pmovq_rr src dst,Pmovq_rr src dst]"
-value "x64_encodes_suffix [Pmovq_rr src dst,Pmovq_rr src dst]"
 value "x64_encodes2 [Pmovq_rr src dst,Pmovq_rr src dst]"
-value "x64_encodes_suffix []"
 value "x64_encodes2 []"
+
+
+
 
 
 end
