theory/x64Semantics.thy
@@ -43,8 +43,10 @@ definition exec_pop :: "usize \<Rightarrow> u64 \<Rightarrow> memory_chunk \<Rig
     let addr = (rs SP) in
       case Mem.loadv chunk m addr of
         None \<Rightarrow> Stuck |
-        Some (Vlong v) => let rs1 = rs#rd <- v in
-          Next (pc + sz) (rs1# SP <- nsp) m
+        Some x => 
+          (case x of Vlong v \<Rightarrow> let rs1 =rs # SP <- nsp  in
+          Next (pc + sz) (rs1#rd <- v ) m |
+                     _ \<Rightarrow> Stuck)
 )"
 
 definition exec_push :: "usize \<Rightarrow> u64 \<Rightarrow> memory_chunk \<Rightarrow> mem \<Rightarrow> regset \<Rightarrow> usize \<Rightarrow> outcome" where
@@ -60,8 +62,8 @@ definition exec_instr :: "instruction \<Rightarrow> u64 \<Rightarrow> u64 \<Righ
   case i of
   Paddq_rr  rd r1 \<Rightarrow> Next (pc + sz) (rs#rd <- ((rs rd) + (rs r1))) m |
   Pret            \<Rightarrow> exec_ret M64 m rs |
-  Ppopl     rd    \<Rightarrow> exec_pop pc sz M32 m rs rd |
-  Ppushl_r  r1    \<Rightarrow> exec_push pc sz M32 m rs (rs r1) |
+  Ppopl     rd    \<Rightarrow> exec_pop pc sz M64 m rs rd |
+  Ppushl_r  r1    \<Rightarrow> exec_push pc sz M64 m rs (rs r1) |
   Pmovq_rr rd r1  \<Rightarrow> Next (pc + sz) (rs#rd <- (rs r1)) m |
   Pmulq_r   r1    \<Rightarrow> let rs1 = rs#RAX <- ((rs RAX)*(rs r1)) in
                      Next (pc + sz) (rs1# RDX <-( (rs RAX)*(rs r1) div (2 ^ 32))) m 
@@ -111,6 +113,504 @@ fun x64_sem :: "nat \<Rightarrow> x64_bin \<Rightarrow> outcome \<Rightarrow> ou
     x64_sem n l (exec_instr ins (of_nat sz) pc rs m)
 )"
 
+
+
+fun interp3 :: "instruction list \<Rightarrow> outcome \<Rightarrow> outcome" where
+"interp3 [] s = s" |
+"interp3 (ins#l) st = (
+  case st of
+  Stuck \<Rightarrow> Stuck |
+  Next pc rs m \<Rightarrow> 
+    interp3 l (exec_instr ins 1 pc rs m)
+)"
+
+fun interp2 :: "instruction list \<Rightarrow> nat list \<Rightarrow> outcome \<Rightarrow> outcome" where
+"interp2 [] _ s = s" |
+"interp2 _ [] s = s" |
+"interp2 (ins#l) (x#xs) st = (
+  case st of
+  Stuck \<Rightarrow> Stuck |
+  Next pc rs m \<Rightarrow> 
+    interp2 l xs (exec_instr ins (of_nat x) pc rs m)
+)"
+
+fun interp1 :: "(nat \<times> instruction) list \<Rightarrow> outcome \<Rightarrow> outcome" where
+"interp1 [] s = s" |
+"interp1 (x#xs) st = (
+  case st of
+  Stuck \<Rightarrow> Stuck |
+  Next pc rs m \<Rightarrow> 
+    let sz = fst x; ins = snd x in
+    interp1 xs (exec_instr ins (of_nat sz) pc rs m)
+)"
+
+definition x64_sem2 :: "nat \<Rightarrow> x64_bin \<Rightarrow> outcome \<Rightarrow> outcome" where
+"x64_sem2 num l st = 
+  (case st of Stuck \<Rightarrow> Stuck |
+     (Next pc rs m) \<Rightarrow>
+      (case x64_decodes_aux num (unat pc) l of
+          None \<Rightarrow> Stuck |
+          Some xs \<Rightarrow> interp1 xs st
+))"
+
+(*
+"x64_sem 0 _ st = st" 
+"x64_sem _ _ Stuck = Stuck" 
+
+definition x64_sem2 :: "nat \<Rightarrow> x64_bin \<Rightarrow> outcome \<Rightarrow> outcome" where
+"x64_sem2 num l st = 
+  (case st of Stuck \<Rightarrow> Stuck |
+     (Next pc rs m) \<Rightarrow>
+      (case x64_decodes_aux num (unat pc) l of
+          None \<Rightarrow> Stuck |
+          Some xs \<Rightarrow> interp3 (map snd xs) st
+))"
+*)
+
+
+
+definition match_stack :: "regset \<Rightarrow> mem \<Rightarrow> bool" where
+"match_stack xrs m = (
+  \<exists> v. Mem.loadv M64 m ((xrs SP) + (u64_of_memory_chunk M64)) = Some (Vlong v))"
+
+definition corr_state:: "outcome \<Rightarrow> outcome \<Rightarrow> bool" where
+"corr_state bst1 bst2 \<equiv> 
+  (case bst1 of
+      Next xpc xrs xm \<Rightarrow>
+        (case bst2 of 
+           Next xpc2 xrs2 xm2 \<Rightarrow>
+            (xrs = xrs2) \<and> xm = xm2 |
+           _ \<Rightarrow> False)|
+      _ \<Rightarrow> False)"
+
+
+
+(*
+lemma interp1_increase_pc:
+  "interp1 [ins] (Next pc rs m) = (Next pc1 rs1 m1 ) \<Longrightarrow>
+  pc1 = pc + of_nat (fst ins)"
+  using exec_instr_def apply(cases "(Next pc rs m)",simp_all)
+  subgoal for x11 apply(unfold exec_instr_def Let_def)
+    apply(cases "snd ins",simp_all)
+      apply(unfold exec_ret_def Let_def)
+    apply(cases "loadv M64 m (rs SP + u64_of_memory_chunk M64)",simp_all)
+    subgoal for a apply(cases a,simp_all)
+      sorry
+    subgoal for x3 apply(unfold exec_push_def Let_def)
+      by(cases "storev M64 m (rs SP - u64_of_memory_chunk M64) (Vlong (rs x3))",simp_all)
+    subgoal for x4 apply(unfold exec_pop_def Let_def)
+      apply(cases "loadv M64 m (rs SP)",simp_all)
+      subgoal for a by(cases a,simp_all)
+      done
+    done
+  done
+
+(*lemma x64_decodes_aux_induct3:"
+  x64_decode (unat pc) xs = Some res1 \<Longrightarrow>
+  len = (fst res1) \<Longrightarrow>
+  x64_decodes_aux n (unat (pc + of_nat len)) xs = Some res2 \<Longrightarrow>
+  x64_decodes_aux n (unat pc) (drop len xs) = Some res3 \<Longrightarrow> 
+  res2 = res3"
+  sorry
+*)
+
+lemma x64_decodes_aux_induct3:"
+  x64_decode (unat pc) xs = Some res1 \<Longrightarrow>
+  len = (fst res1) \<Longrightarrow>
+  x64_decodes_aux n (unat (pc + of_nat len)) xs = 
+  x64_decodes_aux n (unat pc) (drop len xs) "
+  sorry
+
+
+lemma x64_sem2_induct_aux1:
+  "x64_sem2 (Suc num) l st = Next pc' rs' m' \<Longrightarrow>
+   x64_sem2 1 l st = st' \<Longrightarrow>
+   x64_sem2 num l st' = Next pc' rs' m' "
+proof-
+  assume a0:"x64_sem2 (Suc num) l st = Next pc' rs' m'" and
+    a1:"x64_sem2 1 l st = st'"
+  have b0:"st \<noteq> Stuck" using a0 x64_sem2_def by auto
+  have "\<exists> pc rs m. Next pc rs m = st" using b0 by (metis outcome.exhaust)
+  then obtain pc rs m where b1:"Next pc rs m = st" by auto
+  have "x64_sem2 (Suc num) l st = Next pc' rs' m' \<longrightarrow> x64_decodes_aux (Suc num) (unat pc) l \<noteq> None" 
+    using x64_sem2_def
+    apply(cases st) using b1
+    apply(cases "x64_decodes_aux (Suc num) (unat pc) l",simp_all) 
+    apply auto[1] by auto
+  hence b2:"x64_decodes_aux (Suc num) (unat pc) l \<noteq> None" using a0 by blast
+
+  have "\<exists> res. Some res = x64_decodes_aux (Suc num) (unat pc) l"
+    by (meson b2 option.collapse)
+  then obtain res where b3:"Some res = x64_decodes_aux (Suc num) (unat pc) l" by auto
+  have b4:"x64_decode (unat pc) l \<noteq> None"
+    by (metis (no_types, lifting) b2 option.simps(4) x64_decodes_aux.simps(2))
+  hence "\<exists> res1. x64_decode (unat pc) l = Some res1" by blast
+  then obtain res1 where b4:"x64_decode (unat pc) l = Some res1" by auto
+  let "?len" = "fst res1"
+  have "\<exists> res2. x64_decodes_aux num (unat pc) (drop ?len l) = Some res2 \<and> res = res1#res2"
+    using x64_decodes_aux_induct2 b3 b4 by auto
+  then obtain res2 where b5:"x64_decodes_aux num (unat pc) (drop ?len l) = Some res2 \<and> res = res1#res2" by auto
+
+  have c0:"x64_sem2 1 l st = interp1 [res1] st" using b4 x64_sem2_def b1 by auto
+  have c1:"st' \<noteq> Stuck" using a0 sorry
+  have c1_1:"interp1 [res1] st = st'" using c0 a1 by simp
+
+
+  have "\<exists> pc1 rs1 m1. Next pc1 rs1 m1 = st'" using c1 by (metis outcome.exhaust)
+  then obtain pc1 rs1 m1 where c2_1:"Next pc1 rs1 m1 = st'" by auto
+  have c2_2:"pc1 = pc + of_nat (fst res1)" using interp1_increase_pc b1 c2_1 b4 c1_1 by auto
+  (*have "x64_decodes_aux num (unat pc) (drop ?len l) \<noteq> None" sorry*)
+  hence c2_3:"x64_decodes_aux num (unat pc1) l = x64_decodes_aux num (unat pc) (drop ?len l)" 
+    using x64_decodes_aux_induct3 c2_2 b4 b5 by blast
+  have c2_4:"x64_sem2 num l st' = 
+      (case x64_decodes_aux num (unat pc1) l of
+          None \<Rightarrow> Stuck |
+          Some xs \<Rightarrow> interp1 xs st')" using x64_sem2_def c2_1 by auto 
+  hence "x64_sem2 num l st' =  (case x64_decodes_aux num (unat pc) (drop ?len l) of
+          None \<Rightarrow> Stuck |
+          Some xs \<Rightarrow> interp1 xs st')" using c2_3 by simp
+  hence c2:"x64_sem2 num l st' =  interp1 res2 st'" using b5 by simp
+  have c3:"x64_sem2 (Suc num) l st = interp1 res st" using b1 b3 by (metis option.case(2) outcome.simps(4) x64_sem2_def)
+  have c4:"interp1 res2 (interp1 [res1] st) = interp1 (res1#res2) st" using b1 by force
+  thus ?thesis using c0 c1 c1_1 c2 c3 c4 a0 b5 by argo
+qed
+
+
+lemma x64_sem2_induct:
+  "x64_sem2 (Suc num) l st = st2 \<Longrightarrow>
+  \<exists> st'. x64_sem2 1 l st = st' \<and> x64_sem2 num l st' = st2"
+  using x64_sem2_induct_aux1 sorry
+
+
+lemma x64_sem_and_sem2_match_reg_and_mem:
+ "x64_sem num l st = Next pc1 rs1 m1 \<Longrightarrow>
+  x64_sem2 num l st = Next pc2 rs2 m2  \<Longrightarrow>
+  pc1 = pc2 \<and> rs1 = rs2 \<and> m1 = m2"
+proof(induct num arbitrary: l st pc1 rs1 m1 pc2 rs2 m2)
+  case 0
+  then show ?case using x64_sem2_def by simp
+next
+  case (Suc num)
+  assume assm1:"x64_sem (Suc num) l st = Next pc1 rs1 m1" and
+         assm2:"x64_sem2 (Suc num) l st = Next pc2 rs2 m2" 
+  have b0_1:"st \<noteq> Stuck" using assm1 by auto
+  have b0_2:"\<exists> pc rs m. Next pc rs m = st" using b0_1 by (metis outcome.exhaust)
+  then obtain pc rs m where b0_3:"Next pc rs m = st" by auto
+  have "x64_sem2 (Suc num) l st = Next pc2 rs2 m2 \<longrightarrow> x64_decodes_aux (Suc num) (unat pc) l \<noteq> None" 
+    using x64_sem2_def
+    apply(cases st) using b0_3
+    apply(cases "x64_decodes_aux (Suc num) (unat pc) l",simp_all) 
+    apply auto[1] by blast
+  hence b0:"x64_decodes_aux (Suc num) (unat pc) l \<noteq> None" using assm2 by blast
+
+  have "\<exists> res. Some res = x64_decodes_aux (Suc num) (unat pc) l"
+    by (meson b0 option.collapse)
+  then obtain res where b1_0:"Some res = x64_decodes_aux (Suc num) (unat pc) l" by auto
+  have "x64_decode (unat pc) l \<noteq> None" using assm1 b0_3 apply(cases "x64_decode (unat pc) l")  
+    apply simp 
+    apply auto[1]
+    by blast
+  hence "\<exists> res1. x64_decode (unat pc) l = Some res1" by blast
+  then obtain res1 where b1_1:"x64_decode (unat pc) l = Some res1" by auto
+  let "?len" = "fst res1"
+  have "\<exists> res2. x64_decodes_aux num (unat pc) (drop ?len l) = Some res2 \<and> res = res1#res2"
+    using x64_decodes_aux_induct2 b1_0 b1_1 by auto
+  then obtain res2 where b1:"x64_decodes_aux num (unat pc) (drop ?len l) = Some res2 \<and> res = res1#res2" by auto
+
+  have b2_0:"res = res1#res2" using b1 by blast
+  have b2_1:"interp1 res st = Next pc2 rs2 m2"
+    using assm2 x64_sem2_def b1_0
+    by (metis b0_3 option.simps(5) outcome.simps(4))
+  let "?st'" = "interp1 [res1] st"
+  have b2_2:"interp1 res2 ?st' = Next pc2 rs2 m2" using b1
+    using b0_3 b2_1 by force
+  have b2_3:"?st' \<noteq> Stuck" using b2_2 apply(cases ?st',simp_all)
+    apply(cases st,simp_all)
+    subgoal for x11 x12 x13 apply(unfold exec_instr_def)
+      apply(cases "snd res1",simp_all)
+      apply (metis interp1.elims outcome.simps(3) outcome.simps(5))
+       apply (metis interp1.elims outcome.simps(3) outcome.simps(5))
+      by (metis interp1.elims outcome.simps(3) outcome.simps(5))
+    using b0_1 by auto
+
+  (*have "?st' = x64_sem 1 l st" using assm1 b0_3 
+    by (metis (mono_tags, lifting) One_nat_def b1_1 case_prod_beta interp1.simps(1) interp1.simps(2) option.simps(5) outcome.simps(4) x64_sem.simps(1) x64_sem.simps(3))*)
+
+  have c0_1:"?st' = x64_sem2 1 l st" using b0_3 assm2 b1_1 x64_sem2_def by fastforce
+  let "?st2'" = "(exec_instr (snd res1) (of_nat (fst res1)) pc rs m)"
+  have c0_2:"?st2' = x64_sem 1 l st" using assm1 b0_3 b1_1
+    by (metis (mono_tags, lifting) One_nat_def case_prod_beta option.simps(5) x64_sem.simps(1) x64_sem.simps(3))
+  have c0:"x64_sem2 1 l st = x64_sem 1 l st" using b0_3 c0_1 c0_2 by fastforce
+
+  have c1_1:"x64_sem num l ?st2' = Next pc1 rs1 m1" using assm1 b1_1
+    by (metis (no_types, lifting) b0_3 case_prod_conv option.simps(5) split_pairs x64_sem.simps(3))
+  have c1_2:"x64_sem2 num l ?st' = Next pc2 rs2 m2" 
+    using x64_sem2_induct assm2 b2_2 b1 x64_sem2_def b2_3 c0_1 by force
+  have "pc1 = pc2 \<and> rs1 = rs2 \<and> m1 = m2" using c1_1 c1_2 Suc.hyps c0 c0_1 c0_2 by auto
+  then show ?case by simp
+qed
+
+(*lemma x64_sem_and_sem2_match_reg_and_mem2:
+ "x64_sem num l st = st1 \<Longrightarrow>
+  x64_sem2 num l st = st2  \<Longrightarrow>
+  st1 = Stuck \<longrightarrow> st2 = Stuck"
+  sorry*)
+
+(*lemma x64_sem_and_sem2_corr_state:
+  "x64_sem num l st = st1 \<Longrightarrow>
+  x64_sem2 num l st = st2  \<Longrightarrow>
+  corr_state st1 st2"
+  using corr_state_def x64_sem_and_sem2_match_reg_and_mem
+  apply(cases "st1",simp_all)
+   apply(cases "st2",simp_all)
+  subgoal for pc1 rs1 m1*)
+
+lemma x64_sem_and_sem2_corr_state:
+  "x64_sem num l st = Next pc1 rs1 m1 \<Longrightarrow>
+  x64_sem2 num l st = Next pc2 rs2 m2  \<Longrightarrow>
+  corr_state (Next pc1 rs1 m1) (Next pc2 rs2 m2)"
+  using corr_state_def x64_sem_and_sem2_match_reg_and_mem
+  by(cases "Next pc1 rs1 m1",simp_all)
+*)
+
+lemma x64_sem_add_stuck : 
+" x64_sem (m + n) x64_prog Stuck = xst' \<Longrightarrow>
+  x64_sem n x64_prog (x64_sem m x64_prog Stuck) = xst'"
+  apply (cases m,simp)
+  subgoal for m
+    apply(cases n,simp)                
+    by auto
+  done
+
+lemma x64_sem_add: 
+  "x64_sem (m+n) x64_prog xst = xst' \<Longrightarrow>
+    xst = (Next pc rs ms) \<Longrightarrow>
+    \<exists> xst1.
+    x64_sem m x64_prog xst = xst1 \<and> 
+    x64_sem n x64_prog xst1 = xst'"
+  apply (induction m arbitrary: n x64_prog xst xst' pc rs ms)
+  subgoal by simp
+  subgoal for m n x64_prog xst xst' pc rs ms
+    apply simp
+    apply (cases "x64_decode (unat pc) x64_prog"; simp)
+    subgoal by (cases n; simp)
+    subgoal for ins1
+      apply (cases ins1; simp)
+      subgoal for sz ins
+        apply (cases "(exec_instr ins (word_of_nat sz) pc rs ms)"; simp)
+        apply (erule x64_sem_add_stuck)
+        done
+      done
+    done
+  done
+(*
+lemma x64_sem_and_sem2_match_reg_and_mem2:
+ "x64_sem num l st = st1 \<Longrightarrow>
+  x64_sem2 num l st = st2  \<Longrightarrow>
+  st1 = Stuck \<Longrightarrow> st2 = Stuck"
+proof(induct num arbitrary: l st st1 st2)
+  case 0
+  then show ?case using x64_sem2_def by simp
+next
+  case (Suc num)
+  assume assm1:"x64_sem (Suc num) l st = st1" and
+         assm2:"x64_sem2 (Suc num) l st = st2" and
+         assm3:"st1 = Stuck"
+  have b0_1:"st \<noteq> Stuck \<or> st = Stuck" by auto
+  thus ?case
+  proof(cases "st = Stuck")
+    case True
+    then show ?thesis using True apply(cases st,simp_all)
+      using assm2 x64_sem2_def by auto
+  next
+    case False
+    have b0_2:"\<exists> pc rs m. Next pc rs m = st" using b0_1 False by (metis outcome.exhaust)
+    then obtain pc rs m where b0_3:"Next pc rs m = st" by auto
+    let "?st'" = "x64_sem 1 l st"
+    have b1:"?st' = Stuck \<or> ?st' \<noteq> Stuck" by simp
+    thus ?thesis
+    proof(cases "?st' = Stuck")
+      case True
+      have b2:"(x64_decode (unat pc) l = None) \<or> (\<exists> sz ins. x64_decode (unat pc) l = Some(sz,ins) \<and> x64_sem 0 l (exec_instr ins (of_nat sz) pc rs m) = Stuck)" 
+        by (metis (mono_tags, lifting) One_nat_def True b0_3 case_prod_beta option.case_eq_if option.exhaust_sel split_pairs x64_sem.simps(3))
+      thus ?thesis
+      proof(cases "x64_decode (unat pc) l = None")
+        case True
+        have c0:"x64_decodes_aux (Suc num) (unat pc) l = None" using True apply(cases "x64_decode (unat pc) l") apply simp by auto
+        have c1:"x64_sem2 (Suc num) l st = Stuck" using c0 x64_sem2_def apply(cases st,simp_all) using b0_3 by force
+        then show ?thesis using assm2 by blast
+      next
+        case False
+        have c0:"(\<exists> sz ins. x64_decode (unat pc) l = Some(sz,ins) \<and> x64_sem 0 l (exec_instr ins (of_nat sz) pc rs m) = Stuck)" using False b2 by auto
+        then obtain sz ins where c1:"x64_decode (unat pc) l = Some(sz,ins) \<and> x64_sem 0 l (exec_instr ins (of_nat sz) pc rs m) = Stuck" by auto
+        hence c2:"exec_instr ins (of_nat sz) pc rs m = Stuck" by simp
+        have c3:"interp1 [(sz,ins)] st = Stuck" using c2 b0_3 by(cases st,simp_all)
+        have c4:"x64_decodes_aux 1 (unat pc) l = Some [(sz,ins)]" using c1 by simp
+        have c5:"x64_sem2 1 l st = Stuck" using c3 b0_3 x64_sem2_def c4 by(cases st,simp_all) 
+        let "?st2'" = "x64_sem2 1 l st"
+        have c6:"x64_sem2 num l ?st2' = st2" 
+          using x64_sem2_induct assm2 b0_3 by simp
+        have c7:"st2 = Stuck" using c6 c5 x64_sem2_def by auto
+        then show ?thesis using c6 c7 by blast
+      qed
+    next
+      case False
+      have d0:"x64_sem num l ?st' = st1"
+        by (metis assm1 b0_3 plus_1_eq_Suc x64_sem_add)
+      let "?st2'" = "x64_sem2 1 l st"
+      have d0_1:"(x64_decode (unat pc) l \<noteq> None)" using False b0_3  apply(cases st,simp_all) 
+        by (smt (verit) option.case_eq_if x64_decode_def) 
+      have d1_0:"the (x64_decodes_aux 1 (unat pc) l) = [the (x64_decode (unat pc) l)]" apply(cases "x64_decode (unat pc) l",simp_all)  using d0_1 by fastforce
+      have d1:"?st2' \<noteq> Stuck" using x64_sem2_def d0_1 d1_0 apply(cases st,simp_all) apply(cases "x64_decodes_aux 1 (unat pc) l",simp_all) 
+        apply auto[1] 
+        apply (smt (verit) False One_nat_def b0_3 case_prod_conv interp1.elims list.distinct(1) list.inject option.simps(5) outcome.inject outcome.simps(4) split_pairs x64_sem.simps(1) x64_sem.simps(3))
+        apply(cases "x64_decode (unat pc) l",simp_all) 
+        subgoal for a 
+          apply(cases st,simp_all) using b0_3 by blast 
+        done
+        have d2:"x64_sem2 num l ?st2' = st2" using x64_sem2_induct assm2 by presburger
+      have d3:"?st2' = ?st'" using x64_sem_and_sem2_match_reg_and_mem d1 False
+        by (smt (verit, del_insts) outcome.exhaust)
+      have "st2 = Stuck" using d0 d1 d2 d3 assm3 by (metis Suc.hyps)
+      then show ?thesis by simp
+    qed
+  qed
+qed
+
+lemma interp3_equals_interp1:
+  "interp3 (map snd xs) st1 = Next pc1 rs1 m1 \<Longrightarrow> 
+  interp1 xs st2 = Next pc2 rs2 m2 \<Longrightarrow>
+  st1 = Next x1 rs m \<Longrightarrow>
+  st2 = Next y1 rs m \<Longrightarrow>
+  rs1 = rs2 \<and> m1 = m2"
+proof(induct xs arbitrary:st1 pc1 rs1 m1 st2 pc2 rs2 m2 x1 rs m y1)
+  case Nil
+  then show ?case by simp
+next
+  case (Cons a xs)
+  assume a0:"interp3 (map snd (a # xs)) st1 = Next pc1 rs1 m1" and
+  a1:"interp1 (a # xs) st2 = Next pc2 rs2 m2" and
+  a2:"st1 = Next x1 rs m" and
+  a3:"st2 = Next y1 rs m"
+
+  let "?res1" = "interp1 [a] (Next y1 rs m)"
+  let "?res3" = "interp3 [snd a] (Next x1 rs m)"
+  have "?res3 \<noteq> Stuck" using a0 by (smt (verit, best) a2 interp3.elims list.distinct(1) list.inject list.simps(9) outcome.distinct(1) outcome.simps(4) outcome.simps(5))
+  hence "\<exists> pc' rs' m'. Next pc' rs' m' = interp3 [snd a] (Next x1 rs m)"  by (metis outcome.exhaust)
+  then obtain pc' rs' m' where c0:"Next pc' rs' m' = interp3 [snd a] (Next x1 rs m)" by auto
+  have "?res1 \<noteq> Stuck" using a0 
+    by (smt (verit) Cons.prems(2) a3 interp1.elims list.distinct(1) list.sel(3) nth_Cons_0 outcome.simps(3) outcome.simps(4) outcome.simps(5))
+  hence "\<exists> pc'' rs'' m''. Next pc'' rs'' m'' = interp1 [a] (Next y1 rs m)"  by (metis outcome.exhaust)
+  then obtain pc'' rs'' m'' where c1:"Next pc'' rs'' m'' = interp1 [a] (Next y1 rs m)" by auto
+  have c2:"rs' = rs'' \<and> m' = m''" using c1 c0 a2 a3 apply(cases st1,simp_all) apply(cases st2,simp_all)
+    subgoal for x11 apply(unfold exec_instr_def)
+      apply(cases "snd a",simp_all)
+        apply(unfold exec_ret_def Let_def)
+        apply(cases "loadv M64 m (rs SP + u64_of_memory_chunk M64)",simp_all)
+      subgoal for aa by(cases aa,simp_all)
+      subgoal for x3 apply(unfold exec_push_def Let_def)
+        by(cases "storev M64 m (rs SP - u64_of_memory_chunk M64) (Vlong (rs x3))",simp_all)
+      subgoal for x4 apply(unfold exec_pop_def Let_def)
+        apply(cases "loadv M64 m (rs SP)",simp_all)
+        subgoal for aa by(cases aa,simp_all)
+        done
+      done
+    done
+  have d0:"interp3 (map snd xs) (Next pc' rs' m') = Next pc1 rs1 m1" using a0 c0 Cons.prems(3) by auto
+  have d1:"interp1 xs (Next pc'' rs'' m'') = Next pc2 rs2 m2" using a1 c1 Cons.prems(4) by auto
+  have "rs1 = rs2 \<and> m1 = m2" using Cons d0 d1 a0 a1 a2 a3 using c2 by blast
+  then show ?case by auto
+qed
+
+lemma interp1_and_interp3_corr_state:
+  "interp3 (map snd xs) st1 = Next pc1 rs1 m1 \<Longrightarrow> 
+  interp1 xs st2 = Next pc2 rs2 m2 \<Longrightarrow>
+  st1 = Next x1 rs m \<Longrightarrow>
+  st2 = Next y1 rs m \<Longrightarrow>
+  corr_state (Next pc1 rs1 m1) (Next pc2 rs2 m2)"
+  using corr_state_def interp3_equals_interp1
+  by(cases "Next pc1 rs1 m1",simp_all)
+
+
+lemma interp3_equals_interp1_2:
+ "interp3 (map snd xs) st1 = st1' \<Longrightarrow>
+  interp1 xs st2 = st2'  \<Longrightarrow>
+  st1 = Next x1 rs m \<Longrightarrow>
+  st2 = Next y1 rs m \<Longrightarrow>
+  st2' = Stuck \<Longrightarrow> st1' = Stuck"
+proof(induct xs arbitrary:st1 st1' st2 st2' x1 rs m y1)
+  case Nil
+  then show ?case by simp
+next
+  case (Cons a xs)
+  assume a0:"interp3 (map snd (a # xs)) st1 = st1'" and
+  a1:"interp1 (a # xs) st2 = st2'" and
+  a2:"st1 = Next x1 rs m" and
+  a3:"st2 = Next y1 rs m" and
+  a4:"st2' = Stuck"
+
+  let "?res1" = "interp1 [a] (Next y1 rs m)"
+  let "?res3" = "interp3 [snd a] (Next x1 rs m)"
+  have "?res1 = Stuck \<or> ?res1 \<noteq> Stuck" by simp
+  thus ?case
+  proof(cases "?res1 = Stuck")
+    case True
+    have b0:"?res3 = Stuck" 
+      apply(cases a,simp_all) 
+      apply(unfold exec_instr_def)subgoal for aa b apply(cases b,simp_all)
+        using True exec_instr_def apply auto[1] 
+            apply(unfold exec_ret_def Let_def) 
+            apply(cases "loadv M64 m (rs SP + u64_of_memory_chunk M64) ",simp_all)
+        subgoal for ab apply(cases ab,simp_all)
+          subgoal for x5 
+            using True exec_instr_def exec_ret_def by fastforce
+          done
+        subgoal for x3 apply(unfold exec_push_def Let_def)
+          apply(cases "storev M64 m (rs SP - u64_of_memory_chunk M64) (Vlong (rs x3))",simp_all)
+          using True exec_instr_def exec_push_def by force
+        subgoal for x4 apply(unfold exec_pop_def Let_def)
+          apply(cases "loadv M64 m (rs SP)",simp_all)
+          subgoal for ab apply(cases ab,simp_all)
+            subgoal for x5 using True exec_instr_def exec_pop_def by force
+            done
+          done
+        subgoal for x51 x52 using True exec_instr_def by simp
+        subgoal for x6 using True exec_instr_def by simp
+        done
+      done
+    have b1:"interp3 (map snd xs) ?res3 = Stuck" using b0 apply(cases ?res3,simp_all) 
+            by (metis (no_types, lifting) interp3.elims outcome.simps(5))
+    thus ?thesis using Cons.prems(1) Cons.prems(3) by fastforce
+  next
+    case False
+    have c0:"?res1 \<noteq> Stuck" using False by simp
+    have "\<exists> pc'' rs'' m''. Next pc'' rs'' m'' = interp1 [a] (Next y1 rs m)" using False by (metis outcome.exhaust)
+    then obtain pc'' rs'' m'' where c1:"Next pc'' rs'' m'' = interp1 [a] (Next y1 rs m)" by auto
+    have c2:"interp1 xs (Next pc'' rs'' m'') = st2'" using a1 c1 Cons.prems(4) by auto
+    have "\<exists> pc' rs' m'. Next pc' rs' m' = interp3 [snd a] (Next x1 rs m)" using c1 
+    apply(cases a,simp_all) 
+      apply(unfold exec_instr_def)subgoal for aa b apply(cases b,simp_all)
+        using False exec_instr_def apply auto[1] 
+        subgoal for x3 apply(unfold exec_push_def Let_def)
+          apply(cases "storev M64 m (rs SP - u64_of_memory_chunk M64) (Vlong (rs x3))",simp_all)
+          using False exec_instr_def exec_push_def done
+        subgoal for x4 apply(unfold exec_pop_def Let_def)
+          apply(cases "loadv M64 m (rs SP)",simp_all)
+          subgoal for ab apply(cases ab,simp_all) done
+          done
+        done
+      done
+    then obtain pc' rs' m' where c3:"Next pc' rs' m' = interp3 [snd a] (Next x1 rs m)" by auto
+    have c4:"interp3 (map snd xs) (Next pc' rs' m') = st1'" 
+      using Cons.prems(1) Cons.prems(3) c3 by auto
+    have "st1' = Stuck" using Cons c3 c4 
+      by (metis c1 c2 interp3_equals_interp1 list.simps(8) list.simps(9))
+    thus ?thesis by blast
+  qed
+qed
+
+*)
+
 fun x64_sem1 :: "nat \<Rightarrow> u64 \<Rightarrow> (nat \<times> u64 \<times> x64_bin) list \<Rightarrow> outcome \<Rightarrow> outcome" where
 "x64_sem1 0 _ _ st = (let xst_temp =
    case st of
@@ -125,100 +625,9 @@ fun x64_sem1 :: "nat \<Rightarrow> u64 \<Rightarrow> (nat \<times> u64 \<times> 
   let xst' = x64_sem num l xst_temp in (
     x64_sem1 n (pc+off) lt xst'))"
 
-(*
-definition init_reg_map :: "regset" where
-"init_reg_map = (\<lambda> _. 0) (RAX:= 0b00000011, RBX:= 0b00000001)"
-
-definition init_map::"mem" where
-"init_map = Map.empty"
-
-value "init_reg_map RBX"
-
-value "init_reg_map RCX"
-
-value "init_mem 0"
-
-value "x64_sem 2 [0b01001000,0b00000001,0b11011000,0b11000011] (Next (0::u64) (init_reg_map) m)"
-value "x64_sem 1 [0b01001000,0b00000001,0b11011000,0b11000011] (Next (0::u64) (init_reg_map) m)"
-value "x64_sem 0 [0b01001000,0b00000001,0b11011000,0b11000011] (Next (0::u64) (init_reg_map) m)"
-
-value "x64_sem 1 [0b11000011] (Next (0::u64) (init_reg_map) m)"
-
-value "x64_sem 2 [0b11000011] (Next (0::u64) (init_reg_map) m)"
-
-value "x64_sem1 (2::nat) 1 [((1::nat),(1::u64),[0b01001000,0b00000001,0b11011000]),((1::nat),(1::u64),[0b11000011])] (Next (0::u64) (init_reg_map) m)"
-
-lemma "x64_sem1 (1::nat) 1 [((1::nat),(1::u64),[0b01001000,0b00000001,0b11011000]),((1::nat),(1::u64),[0b11000011])] (Next xpc rs m)  = exec_instr Pret 1 0 rs m "
-  using x64_decode_def by simp*)
-
-fun interp3 :: "instruction list \<Rightarrow> outcome \<Rightarrow> outcome" where
-"interp3 [] s = s" |
-"interp3 (ins#l) st = (
-  case st of
-  Stuck \<Rightarrow> Stuck |
-  Next pc rs m \<Rightarrow> 
-    interp3 l (exec_instr ins 1 pc rs m)
-)"
-
-(*
-fun interp3 :: "instruction list \<Rightarrow> outcome \<Rightarrow> outcome" where
-"interp3 [] s = s" |
-"interp3 (ins#l) st = (
-  case st of
-  Stuck \<Rightarrow> Stuck |
-  Next pc rs m \<Rightarrow> (
-    let x = (x64_encode ins) in
-      case x of None \<Rightarrow> Stuck |
-                Some res \<Rightarrow> 
-          let result = x64_decode 0 res in
-              case result of None \<Rightarrow> Stuck |
-                             Some res \<Rightarrow> let len = fst res
-    in interp3 l (exec_instr ins (of_nat len) pc rs m)
-))"
-
-
-
-fun interp3 :: "instruction list \<Rightarrow> outcome \<Rightarrow> outcome" where
-"interp3 [] s = s" |
-"interp3 (ins#l) st = (
-  case st of
-  Stuck \<Rightarrow> Stuck |
-  Next pc rs m \<Rightarrow> (
-    let len = (case ins of Pret \<Rightarrow> 1 |
-                  Ppopl dst \<Rightarrow> 2 |
-                  Ppushl_r dst \<Rightarrow> 2 |
-                   _ \<Rightarrow> 3 )
-    in interp3 l (exec_instr ins len pc rs m)
-))"
-*)
-value "x64_sem1 0 "
-
-(*definition x64_sem1 ::"nat \<Rightarrow> (nat \<times> x64_bin) list \<Rightarrow> outcome \<Rightarrow> outcome" where
-"x64_sem1 pc lt xst \<equiv> (let (fuel,l) = lt!pc in
-                       let xst_temp = (case xst of (Next xpc rs m) \<Rightarrow> Next 0 rs m | Stuck \<Rightarrow> Stuck) in
-                       let xst' = x64_sem fuel l xst_temp in (xst', pc+1))"*)
-
-value "length [1::nat,2,3]"
-
-(*fun x64_sem1 ::"nat \<Rightarrow> x64_bin \<Rightarrow> outcome \<Rightarrow> (outcome \<times> nat)" where
-"x64_sem1 pc l Stuck = (Stuck, pc)" |
-"x64_sem1 pc l (Next pc rs m) = (case x64_decode (unat pc) l of
-  None \<Rightarrow> Stuck |
-  Some (sz, ins) \<Rightarrow>
-    x64_sem1 n l (exec_instr ins (of_nat sz) pc rs m))"
-*)
-(*
-fun interp3 :: "instruction list \<Rightarrow> outcome \<Rightarrow> outcome" where
-"interp3 [] s = s" |
-"interp3 (ins#l) st = (
-  case st of
-  Stuck \<Rightarrow> Stuck |
-  Next rs m \<Rightarrow> (
-        interp3 l (exec_instr ins 1 rs m)
-))"
-*)
-
 
 type_synonym x64_state = outcome
+
+
 
 end
