theory/Proof1.thy
@@ -5,18 +5,36 @@ imports
 
 begin
 
-value "x64_decode 0 (the (x64_encode (Paddq_rr RAX RBX)))"
+value "x64_decode 0 (x64_encode (Paddq_rr RAX RBX))"
+
+lemma list_in_list_prop_aux1:"x@[] = x"
+  by blast
+
+lemma list_in_list_prop_aux2: "list_in_list l2 (length l1) (l1@l2@l3)"
+  apply (induction l2 arbitrary: l1 l3)
+  subgoal for l1 l3
+    by simp
+  subgoal for a l2 l1 l3
+    apply simp
+    by (metis append.left_neutral append_Cons append_assoc length_append_singleton)
+  done
+
+lemma list_in_list_prop:"list_in_list l 0 l"
+  using list_in_list_prop_aux1
+  by (metis append_Nil list_in_list_prop_aux2 list.size(3))
 
 lemma x64_encode_decode_consistency:
- "Some l_bin = x64_encode ins \<Longrightarrow>
-    x64_decode 0 l_bin = Some (length l_bin, ins)"
- 
-  apply(cases ins,simp_all)
+ "list_in_list l_bin pc l \<Longrightarrow>
+   l_bin = x64_encode ins \<Longrightarrow>
+   x64_decode pc l = Some (length l_bin, ins)"
+  sorry
+  (*apply(cases ins,simp_all)
   subgoal for dst src 
     \<comment> \<open> Paddq_rr \<close> 
     apply (unfold Let_def construct_rex_to_u8_def construct_modsib_to_u8_def)
-    subgoal by (cases src; simp;cases dst; auto simp add: x64_decode_def bitfield_insert_u8_def Let_def ireg_of_u8_def
+    subgoal apply (cases src; simp;cases dst; auto simp add: x64_decode_def bitfield_insert_u8_def Let_def ireg_of_u8_def
           Suc3_eq_add_3 add.commute)
+      done
     done
    apply(unfold x64_decode_def;auto)
   subgoal for dst
@@ -40,7 +58,7 @@ lemma x64_encode_decode_consistency:
     apply (unfold Let_def construct_rex_to_u8_def construct_modsib_to_u8_def)
     apply (cases dst; auto simp add: x64_decode_def bitfield_insert_u8_def Let_def ireg_of_u8_def)
   done
-  done
+  done*)
 
 (*lemma x64_encodes_decodes_consistency:
   "Some l_bin = x64_encodes2 ins \<Longrightarrow>
