theory/Proof2.thy
@@ -2,11 +2,79 @@ theory Proof2
   imports Proof1 x64Semantics rBPFSem
 begin
 
+(*lemma x64_decode_extend:
+  assumes 
+    a1:"x64_decode 0 x = Some res1"
+  shows "x64_decode 0 (x@[a]) = Some res1"
+  apply(unfold x64_decode_def)
+  apply(split if_splits,simp_all)
+  apply (unfold Let_def)
+  apply(split if_splits)+ apply simp_all
+  apply(cases "ireg_of_u8 (bitfield_insert_u8 3 (Suc 0) 4 (and 1 ((x @ [a]) ! 0 >> 2)))",simp_all)
+   apply(cases "ireg_of_u8 (bitfield_insert_u8 3 (Suc 0) (and 7 ((x @ [a]) ! 0)) 0)",simp_all)
+    prefer 2
+  subgoal for aa 
+    apply(cases "ireg_of_u8 (bitfield_insert_u8 3 (Suc 0) (and 7 ((x @ [a]) ! Suc (Suc 0))) (and 1 ((x @ [a]) ! 0))) ",simp_all)
+     apply(cases "ireg_of_u8 (bitfield_insert_u8 3 (Suc 0) (and 7 ((x @ [a]) ! Suc 0)) (and 1 ((x @ [a]) ! 0)))",simp_all)
+      apply(cases"ireg_of_u8 (bitfield_insert_u8 3 (Suc 0) (and 7 ((x @ [a]) ! Suc (Suc 0) >> 3)) (and 1 ((x @ [a]) ! 0 >> 2)))",simp_all)
+       apply rule+
+           apply simp
+          apply auto[1]
+         apply rule
+         apply(unfold bitfield_insert_u8_def Let_def ireg_of_u8_def,simp) 
+    apply(split if_splits)+ 
+              apply simp
+        (*    apply(split if_splits)+  apply simp
+             apply(split if_splits)+  apply simp
+             apply(split if_splits)+  apply simp
+             apply(split if_splits)+  apply simp*)
+             apply simp
+            apply auto[1]
+           apply simp
+    apply simp
+         apply rule+ 
+          apply(split if_splits)+  
+               apply blast
+              apply auto[1]
+             apply simp
+            apply simp
+    apply(split if_splits)+ 
+               apply blast
+              apply blast
+             apply blast
+            apply blast
+           apply(split if_splits)+ 
+               apply blast
+              apply blast
+             apply blast
+            apply blast
+    
+    
+
+
+
+   (*apply(cases "ireg_of_u8 (bitfield_insert_u8 3 (Suc 0) (and 7 ((x @ [a]) ! Suc (Suc 0))) (and 1 ((x @ [a]) ! 0))) ",simp_all)
+    apply(cases "ireg_of_u8 (bitfield_insert_u8 3 (Suc 0) (and 7 ((x @ [a]) ! Suc 0)) (and 1 ((x @ [a]) ! 0)))",simp_all)
+  apply(cases "ireg_of_u8 (bitfield_insert_u8 3 (Suc 0) (and 7 ((x @ [a]) ! Suc (Suc 0) >> 3)) (and 1 ((x @ [a]) ! 0 >> 2))) ",simp_all)*)
+      apply rule+
+         prefer 5
+  subgoal for aa
+    apply rule+ 
+  sorry
+
+
+*)
+  
+
+
 lemma x64_decode_extend:
   assumes 
     a1:"x64_decode 0 x = Some res1"
   shows "x64_decode 0 (x@xs) = Some res1"
-  apply(unfold x64_decode_def)
+  sorry
+
+
+  (*apply(unfold x64_decode_def)
   apply(split if_splits,simp_all)
   apply (unfold Let_def)
  apply(split if_splits)
@@ -23,7 +91,7 @@ lemma x64_decode_extend:
           apply(split if_splits,simp_all)
           apply (simp add: nth_append)
          apply (metis One_nat_def length_greater_0_conv nth_append option.inject option.simps(3))
-  prefer 2 
+  prefer 2 *)
 (*proof-
   have "\<exists> l_bin. x64_encode (snd res1) = Some l_bin" sorry
   then obtain l_bin where b0:"x64_encode (snd res1) = Some l_bin" by auto
@@ -34,9 +102,9 @@ lemma x64_decode_extend:"x\<noteq> [] \<Longrightarrow> x64_decode 0 x = Some re
   sorry
 *)
 
-
+(*
 lemma x64_encodes_decodes_consistency:"
-    Some l_bin = x64_encodes2 ins \<Longrightarrow>
+    l_bin = x64_encodes2 ins \<Longrightarrow>
     x64_decodes_aux (length ins) 0 l_bin = Some ins_list \<Longrightarrow>
     map snd ins_list = ins"
 proof(induct ins arbitrary: l_bin ins_list)
@@ -44,31 +112,25 @@ proof(induct ins arbitrary: l_bin ins_list)
   then show ?case by auto
 next
   case (Cons a prog)
-  assume assm1:"Some l_bin = x64_encodes2 (a # prog)" and
+  assume assm1:"l_bin = x64_encodes2 (a # prog)" and
          assm2:"x64_decodes_aux (length (a # prog)) 0 l_bin = Some ins_list"
-  have "\<exists> l_bin2. Some l_bin2 = x64_encodes2 prog" using Cons x64_encodes2_induct x64_encodes2_def assm1 
+  have "\<exists> l_bin2. l_bin2 = x64_encodes2 prog" using Cons x64_encodes2_induct x64_encodes2_def assm1 
     by (metis (no_types, lifting) option.case_eq_if x64_encodes1.simps(2))
-  then obtain l_bin2 where c0:"Some l_bin2 = x64_encodes2 prog" by auto
-  have "\<exists> l_bin1. Some l_bin1 = x64_encode a" using assm1
+  then obtain l_bin2 where c0:"l_bin2 = x64_encodes2 prog" by auto
+  have "\<exists> l_bin1. l_bin1 = x64_encode a" using assm1
     by (metis (no_types, lifting) option.case_eq_if option.collapse x64_encodes1.simps(2) x64_encodes2_def)
-  then obtain l_bin1 where c1:"Some l_bin1 = x64_encode a" by auto
+  then obtain l_bin1 where c1:"l_bin1 = x64_encode a" by auto
   have c2:"l_bin1@l_bin2 = l_bin" using x64_encodes2_induct c0 c1 assm1 by metis
 
-  have d0_1: "\<exists> ins_list1. x64_decode 0 l_bin1 = Some ins_list1" using x64_encode_decode_consistency c1 by blast
+  have d0_1: "\<exists> ins_list1. x64_decode 0 l_bin1 = Some ins_list1" using x64_encode_decode_consistency c1 list_in_list_prop by blast
   then obtain ins_list1 where d0:"x64_decode 0 l_bin1 = Some ins_list1" by auto
-  have d1:"snd ins_list1 = a" using d0 x64_encode_decode_consistency c1 by auto
-  have d1_1:"l_bin1 \<noteq> []" using c1 apply(cases " x64_encode a",simp_all) 
-    subgoal for aa apply(cases a,simp_all)
-      subgoal for x11 x12 by auto
-          apply auto[1]
+  have d1:"snd ins_list1 = a" using d0 x64_encode_decode_consistency c1 list_in_list_prop by fastforce
+  have d1_1:"l_bin1 \<noteq> []" using c1 apply(cases "x64_encode a",simp_all) 
+    apply(cases a,simp_all)
       subgoal for x3 apply(unfold Let_def) apply (split if_splits) apply auto[1] 
         apply auto[1]
         done
       subgoal for x4 apply(unfold Let_def) apply (split if_splits) apply auto[1] apply auto[1] done
-      subgoal for x51 x52 apply auto[1]
-        done
-      subgoal for x6 by blast
-      done
     done
   have d1_2:"x64_decode 0 l_bin = Some ins_list1" using x64_decode_extend d0 d1 c2 d1_1 by blast
   let "?insx_len" =  "fst ins_list1"
@@ -77,91 +139,12 @@ next
     using x64_decodes_aux_induct2 assm2 d1_2 d2_1
     by (metis One_nat_def add.right_neutral add_Suc_right)
   then obtain ins_list2 where d2:" x64_decodes_aux (length prog) 0 (drop ?insx_len l_bin) = Some ins_list2 \<and> ins_list = ins_list1#ins_list2" by auto
-  have d2_0:"l_bin2 = drop ?insx_len l_bin" using c1 c2 d0 x64_encode_decode_consistency d2 assm1 assm2 by auto
+  have d2_0:"l_bin2 = drop ?insx_len l_bin" using c1 c2 d0 x64_encode_decode_consistency d2 assm1 assm2 list_in_list_prop sorry
   have e0:"map snd ins_list2 = prog" using Cons c0 d2 d2_0 by blast
   have e2:"map snd ins_list = a # prog" using d2 c2 d1 e0 by fastforce
   then show ?case by simp
 qed
-
-
-
-  (*
-lemma "
-    Some l_bin = x64_encodes2 ins \<Longrightarrow>
-    x64_decodes_aux (length ins) 0 l_bin = Some ins_list \<Longrightarrow>
-    map snd ins_list = ins"
-proof(induct ins arbitrary: l_bin ins_list)
-  case Nil
-  then show ?case by auto
-next
-  case (Cons a prog)
-  assume assm1:"Some l_bin = x64_encodes2 (a # prog)" and
-         assm2:"x64_decodes_aux (length (a # prog)) 0 l_bin = Some ins_list"
-  have "\<exists> l_bin2. Some l_bin2 = x64_encodes2 prog" using Cons x64_encodes2_induct x64_encodes2_def assm1 
-    by (metis (no_types, lifting) option.case_eq_if x64_encodes1.simps(2))
-  then obtain l_bin2 where c0:"Some l_bin2 = x64_encodes2 prog" by auto
-  have "\<exists> l_bin1. Some l_bin1 = x64_encode a" using assm1
-    by (metis (no_types, lifting) option.case_eq_if option.collapse x64_encodes1.simps(2) x64_encodes2_def)
-  then obtain l_bin1 where c1:"Some l_bin1 = x64_encode a" by auto
-  have c2:"l_bin1@l_bin2 = l_bin" using x64_encodes2_induct c0 c1 assm1 by metis
-
-  have d_1: "\<exists> ins_list1. x64_decode 0 l_bin1 = Some ins_list1" using x64_encode_decode_consistency c1 by blast
-  hence "\<exists> ins_list1. x64_decode 0 l_bin = Some ins_list1" 
-    by (smt (verit, del_insts) assm2 length_Cons not_None_eq option.case_eq_if x64_decodes_aux.simps(2))
-  then obtain ins_list1 where d0:"x64_decode 0 l_bin = Some ins_list1" by auto
-  have d1:"snd ins_list1 = a" using d0 x64_encode_decode_consistency c1
-    by (smt (z3) One_nat_def Suc_le_mono c2 le_add1 list.size(3) option.discI option.inject plus_1_eq_Suc split_pairs x64_decode_def x64_decode_extend)
-  let "?insx_len" =  "fst ins_list1"
-  have d2_1:"(length prog) + 1 = length (a # prog)" by simp
-  have "\<exists> ins_list2. x64_decodes_aux (length prog) 0 (drop ?insx_len l_bin) = Some ins_list2 \<and> ins_list = ins_list1#ins_list2" 
-    using x64_decodes_aux_induct2 assm2 d0 d2_1
-    by (metis One_nat_def add.right_neutral add_Suc_right)
-  then obtain ins_list2 where d2:" x64_decodes_aux (length prog) 0 (drop ?insx_len l_bin) = Some ins_list2 \<and> ins_list = ins_list1#ins_list2" by auto
-  have d2_0:"l_bin2 = drop ?insx_len l_bin" using c1 c2 d0 x64_encode_decode_consistency d2 assm1 assm2 try
-  (*have "\<exists> ins_list2. x64_decodes_aux (length prog) 0 l_bin2 = Some ins_list2" using assm2 assm1 d2_0 sorry
-  then obtain ins_list2 where d2:"x64_decodes_aux (length prog) 0 l_bin2 = Some ins_list2" by auto
- have "l_bin1 \<noteq> []" using c1 apply(cases " x64_encode a",simp_all) 
-    subgoal for aa apply(cases a,simp_all)
-      subgoal for x11 x12 by auto
-          apply auto[1]
-      subgoal for x3 apply(unfold Let_def) apply (split if_splits) apply auto[1] 
-        apply auto[1]
-        done
-      sorry
-    sorry
-  hence d2_1:"x64_decode 0 l_bin = Some ins_list1" using d0 c2 x64_decode_extend by blast
-  have d2_2:"l_bin1 = (take ?insx_len l_bin) " by (metis append_same_eq c2 d2_0 hhh)
 *)
-  have e0:"map snd ins_list2 = prog" using Cons c0 d2 d2_0 by blast
-  have e2:"map snd ins_list = a # prog" using d2 c2 d1 e0 by fastforce
-  then show ?case by simp
-qed
-
-have "\<exists> insa. x64_encode ins = Some insa"
-    using assm1 option.collapse x64_encodes2_def by fastforce
-  then obtain insa where b2:"x64_encode a = Some insa" by auto
-  hence "\<exists> insx. x64_decode 0 insa = Some insx" by (metis x64_encode_decode_consistency)
-  then obtain insx where b3:"x64_decode 0 insa = Some insx" by auto
-  have b4:"snd insx = a" using x64_encode_decode_consistency b2 b3 by (metis option.sel snd_conv)
-  let "?insx_len" =  "fst insx"
-  have "\<exists> hhh. x64_decodes_aux (length a) 0 insa = Some hhh" using assm2 b2 try
-  have "x64_decodes_aux 1 0 insa = Some [insx]" using x64_decodes_aux_equiv b3 try
-  have "\<exists> ins_list'. x64_decodes_aux (length ins) ?insx_len l_bin' = Some ins_list'" 
-    using b1 assm2 x64_decodes_aux_induct b2 b3 b4
-   
-  then obtain ins_list' where  b2:"x64_decodes 0 l_bin' = Some ins_list'" by auto
-  have b3:"map snd ins_list' = ins" using b0 b1 b2 Cons by blast
-  have "\<exists> h. x64_encode a = Some h"
-    by (metis (mono_tags, lifting) assm1 option.case_eq_if option.collapse x64_encodes_aux.simps(2) x64_encodes_def x64_encodes_suffix_def)
-  then obtain h where "x64_encode a = Some h" by auto
-  moreover have "\<exists> x. x64_decode 0 h = Some x" 
-    by (metis calculation x64_encode_decode_consistency)
-    then obtain x where "x64_decode 0 h = Some x" by auto
-    hence c0:"snd x = a" by (metis calculation option.inject snd_conv x64_encode_decode_consistency)
-  then show ?case using c0 b3 Cons 
-  qed*)
-
-
 
 
 end
